im an idiot

theories/Sound.v
@@ -56,7 +56,7 @@ Module Type SOUND_F(Import Conf : DETECT_CONF)(Import Params : DETECT_PARAMS(Con
 
 
     Lemma SRPC_M_net_AnySrpc [N S n] :
-      net_sane '' N ->
+      net_sane N ->
       NetMod.get n N = S ->
       AnySRPC_serv S.
     Proof.
@@ -84,8 +84,8 @@ Module Type SOUND_F(Import Conf : DETECT_CONF)(Import Params : DETECT_PARAMS(Con
       econstructor 3; iattac.
     Qed.
 
-    Lemma SRPC_M_net_in_net_Q_in_M [N n c v v' MQ0 MQ1 M I P O] :
-      net_sane '' N ->
+    Lemma SRPC_M_net_in_net_Q_in_M [N : MNet] [ n c v v' MQ0 MQ1 M I P O] :
+      net_sane N ->
       NetMod.get n N = mserv (MQ0 ++ TrRecv (c, Q) v :: MQ1) M (serv I P O) ->
       ~ List.In (c, Q, v') (I ++ MQ_r (MQ0 ++ MQ1)).
 
@@ -96,17 +96,17 @@ Module Type SOUND_F(Import Conf : DETECT_CONF)(Import Params : DETECT_PARAMS(Con
       rewrite MQ_r_app.
       remember (MQ_r MQ1) as I1 eqn:x; clear x.
       repeat (rewrite (app_assoc) in * ).
-      remember (&I ++ MQ_r MQ0) as I0 eqn:x; clear x.
+      remember (&I ++ MQ_r MQ0) as I0 eqn:x.
       destruct (Deq_dec' I0 (c, Q)); hsimpl in *.
       - rename Q' into I0'.
-        assert (Deq (c, Q) v0 (I0 ++ (c, Q, v) :: I1) (I0' ++ (c, Q, v) :: I1)) by attac.
-        bs (~ List.In (c, Q, v) (I0' ++ (c, Q, v) :: I1)).
+        assert (Deq (c, Q) v0 ((&I ++ MQ_r MQ0) ++ (c, Q, v) :: I1) (I0' ++ (c, Q, v) :: I1)) by attac.
+        bs (~ List.In (c, Q, v) (I0' ++ (c, Q, v) :: I1)) by attac.
       - assert (Deq (c, Q) v ((c, Q, v) :: I1) I1) by attac.
-        bs (Deq (c, Q) v (I0 ++ (c, Q, v) :: I1) (I0 ++ I1)) by eauto using Deq_app_l_not_Deq.
+        bs (Deq (c, Q) v (_ ++ (c, Q, v) :: I1) (_ ++ I1)) by eauto using Deq_app_l_not_Deq.
     Qed.
 
-    Lemma SRPC_M_net_in_net_Q_in_M0 [N n c v v' MQ0 MQ1 M S] :
-      net_sane '' N ->
+    Lemma SRPC_M_net_in_net_Q_in_M0 [N : MNet] [ n c v v' MQ0 MQ1 M S] :
+      net_sane N ->
       NetMod.get n N = mserv (MQ0 ++ TrRecv (c, Q) v :: MQ1) M S ->
       ~ List.In (TrRecv (c, Q) v') MQ0.
     Proof. intros. destruct S as [I P O].
@@ -114,8 +114,8 @@ Module Type SOUND_F(Import Conf : DETECT_CONF)(Import Params : DETECT_PARAMS(Con
            iattac.
     Qed.
 
-    Lemma SRPC_M_net_in_net_Q_in_M1 [N n c v v' MQ0 MQ1 M S] :
-      net_sane '' N ->
+    Lemma SRPC_M_net_in_net_Q_in_M1 [N : MNet] [ n c v v' MQ0 MQ1 M S] :
+      net_sane N ->
       NetMod.get n N = mserv (MQ0 ++ TrRecv (c, Q) v :: MQ1) M S ->
       ~ List.In (TrRecv (c, Q) v') MQ1.
     Proof. intros. destruct S as [I P O].
@@ -123,8 +123,8 @@ Module Type SOUND_F(Import Conf : DETECT_CONF)(Import Params : DETECT_PARAMS(Con
            iattac.
     Qed.
 
-    Lemma SRPC_M_net_in_net_Q_in_MP [N n c v v' MQ0 MQ1 M I P O] :
-      net_sane '' N ->
+    Lemma SRPC_M_net_in_net_Q_in_MP [N : MNet] [ n c v v' MQ0 MQ1 M I P O] :
+      net_sane N ->
       NetMod.get n N = mserv (MQ0 ++ TrRecv (c, Q) v :: MQ1) M (serv I P O) ->
       ~ List.In (c, Q, v') I.
     Proof. intros.
@@ -132,8 +132,8 @@ Module Type SOUND_F(Import Conf : DETECT_CONF)(Import Params : DETECT_PARAMS(Con
            iattac.
     Qed.
 
-    Lemma SRPC_M_net_in_net_Q_in_P [N n c v v' MQ M I I' P O] :
-      net_sane '' N ->
+    Lemma SRPC_M_net_in_net_Q_in_P [N : MNet] [ n c v v' MQ M I I' P O] :
+      net_sane N ->
       NetMod.get n N = mserv MQ M (serv I P O) ->
       Deq (c, Q) v I I' ->
       ~ List.In (c, Q, v') (I' ++ MQ_r MQ).
@@ -147,8 +147,8 @@ Module Type SOUND_F(Import Conf : DETECT_CONF)(Import Params : DETECT_PARAMS(Con
       iattac.
     Qed.
 
-    Lemma SRPC_M_net_in_net_Q_in_PP [N n c v v' MQ M I I' P O] :
-      net_sane '' N ->
+    Lemma SRPC_M_net_in_net_Q_in_PP [N : MNet] [ n c v v' MQ M I I' P O] :
+      net_sane N ->
       NetMod.get n N = mserv MQ M (serv I P O) ->
       Deq (c, Q) v I I' ->
       ~ List.In (c, Q, v') I'.
@@ -156,8 +156,8 @@ Module Type SOUND_F(Import Conf : DETECT_CONF)(Import Params : DETECT_PARAMS(Con
            assert (~ List.In (c, Q, v') (&I' ++ MQ_r MQ)) by eauto using SRPC_M_net_in_net_Q_in_P.
            iattac.
     Qed.
-    Lemma SRPC_M_net_in_net_Q_in_PM [N n c v v' MQ M I I' P O] :
-      net_sane '' N ->
+    Lemma SRPC_M_net_in_net_Q_in_PM [N : MNet] [ n c v v' MQ M I I' P O] :
+      net_sane N ->
       NetMod.get n N = mserv MQ M (serv I P O) ->
       Deq (c, Q) v I I' ->
       ~ List.In (TrRecv (c, Q) v') MQ.
@@ -166,8 +166,8 @@ Module Type SOUND_F(Import Conf : DETECT_CONF)(Import Params : DETECT_PARAMS(Con
            iattac.
     Qed.
 
-    Lemma SRPC_M_net_in_net_R_in_M [N n s s' v v' MQ0 MQ1 M I P O] :
-      net_sane '' N ->
+    Lemma SRPC_M_net_in_net_R_in_M [N : MNet] [ n s s' v v' MQ0 MQ1 M I P O] :
+      net_sane N ->
       NetMod.get n N = mserv (MQ0 ++ TrRecv (s, R) v :: MQ1) M (serv I P O) ->
       ~ List.In (s', R, v') (I ++ MQ_r (MQ0 ++ MQ1)).
 
@@ -177,19 +177,18 @@ Module Type SOUND_F(Import Conf : DETECT_CONF)(Import Params : DETECT_PARAMS(Con
       unfold net_deinstr, deinstr in *; hsimpl in *.
       remember (MQ_r MQ1) as I1 eqn:x; clear x.
       repeat (rewrite (app_assoc) in * ).
-      remember (&I ++ MQ_r MQ0) as I0 eqn:x; clear x.
-
+      remember (&I ++ MQ_r MQ0) as I0 eqn:x.
       destruct (Deq_dec' I0 (s, R)); hsimpl in *.
       - rename Q' into I0'.
-        assert (Deq (s, R) v0 (I0 ++ (s, R, v) :: I1) (I0' ++ (s, R, v) :: I1)) by attac.
+        assert (Deq (s, R) v0 (_ ++ (s, R, v) :: I1) (I0' ++ (s, R, v) :: I1)) by attac.
         bs (~ List.In (s, R, v) (I0' ++ (s, R, v) :: I1)).
       - assert (Deq (s, R) v ((s, R, v) :: I1) I1) by attac.
-        assert (Deq (s, R) v (I0 ++ (s, R, v) :: I1) (I0 ++ I1)) by eauto using Deq_app_l_not_Deq.
-        bs (~ List.In (s', R, v) (I0 ++ I1)).
+        assert (Deq (s, R) v (_ ++ (s, R, v) :: I1) (_ ++ I1)) by eauto using Deq_app_l_not_Deq.
+        bs (~ List.In (s', R, v) (_ ++ I1)).
     Qed.
 
-    Lemma SRPC_M_net_in_net_R_in_M0 [N n s s' v v' MQ0 MQ1 M S] :
-      net_sane '' N ->
+    Lemma SRPC_M_net_in_net_R_in_M0 [N : MNet] [ n s s' v v' MQ0 MQ1 M S] :
+      net_sane N ->
       NetMod.get n N = mserv (MQ0 ++ TrRecv (s, R) v :: MQ1) M S ->
       ~ List.In (TrRecv (s', R) v') MQ0.
     Proof.
@@ -197,8 +196,8 @@ Module Type SOUND_F(Import Conf : DETECT_CONF)(Import Params : DETECT_PARAMS(Con
       assert (~ List.In (s', R, v') (&I ++ MQ_r (MQ0 ++ MQ1))) by eauto using SRPC_M_net_in_net_R_in_M.
       attac.
     Qed.
-    Lemma SRPC_M_net_in_net_R_in_M1 [N n s s' v v' MQ0 MQ1 M S] :
-      net_sane '' N ->
+    Lemma SRPC_M_net_in_net_R_in_M1 [N : MNet] [ n s s' v v' MQ0 MQ1 M S] :
+      net_sane N ->
       NetMod.get n N = mserv (MQ0 ++ TrRecv (s, R) v :: MQ1) M S ->
       ~ List.In (TrRecv (s', R) v') MQ1.
     Proof.
@@ -206,8 +205,8 @@ Module Type SOUND_F(Import Conf : DETECT_CONF)(Import Params : DETECT_PARAMS(Con
       assert (~ List.In (s', R, v') (&I ++ MQ_r (MQ0 ++ MQ1))) by eauto using SRPC_M_net_in_net_R_in_M.
       attac.
     Qed.
-    Lemma SRPC_M_net_in_net_R_in_MP [N n s s' v v' MQ0 MQ1 M I P O] :
-      net_sane '' N ->
+    Lemma SRPC_M_net_in_net_R_in_MP [N : MNet] [ n s s' v v' MQ0 MQ1 M I P O] :
+      net_sane N ->
       NetMod.get n N = mserv (MQ0 ++ TrRecv (s, R) v :: MQ1) M (serv I P O) ->
       ~ List.In (s', R, v') I.
     Proof.
@@ -216,8 +215,8 @@ Module Type SOUND_F(Import Conf : DETECT_CONF)(Import Params : DETECT_PARAMS(Con
       attac.
     Qed.
 
-    Lemma SRPC_M_net_in_net_R_in_P [N n s s' v v' MQ M I I' P O] :
-      net_sane '' N ->
+    Lemma SRPC_M_net_in_net_R_in_P [N : MNet] [ n s s' v v' MQ M I I' P O] :
+      net_sane N ->
       NetMod.get n N = mserv MQ M (serv I P O) ->
       Deq (s, R) v I I' ->
       ~ List.In (s', R, v') (I' ++ MQ_r MQ).
@@ -230,8 +229,8 @@ Module Type SOUND_F(Import Conf : DETECT_CONF)(Import Params : DETECT_PARAMS(Con
       attac.
     Qed.
 
-    Lemma SRPC_M_net_in_net_R_in_PP [N n s s' v v' MQ M I I' P O] :
-      net_sane '' N ->
+    Lemma SRPC_M_net_in_net_R_in_PP [N : MNet] [ n s s' v v' MQ M I I' P O] :
+      net_sane N ->
       NetMod.get n N = mserv MQ M (serv I P O) ->
       Deq (s, R) v I I' ->
       ~ List.In (s', R, v') I'.
@@ -240,8 +239,8 @@ Module Type SOUND_F(Import Conf : DETECT_CONF)(Import Params : DETECT_PARAMS(Con
       assert (~ List.In (s', R, v') (&I' ++ MQ_r MQ)) by eauto using SRPC_M_net_in_net_R_in_P.
       attac.
     Qed.
-    Lemma SRPC_M_net_in_net_R_in_PM [N n s s' v v' MQ M I I' P O] :
-      net_sane '' N ->
+    Lemma SRPC_M_net_in_net_R_in_PM [N : MNet] [ n s s' v v' MQ M I I' P O] :
+      net_sane N ->
       NetMod.get n N = mserv MQ M (serv I P O) ->
       Deq (s, R) v I I' ->
       ~ List.In (TrRecv (s', R) v') MQ.
@@ -251,8 +250,8 @@ Module Type SOUND_F(Import Conf : DETECT_CONF)(Import Params : DETECT_PARAMS(Con
       attac.
     Qed.
 
-    Lemma SRPC_M_net_in_net_R_in_lock [N n s v MQ M S] :
-      net_sane '' N ->
+    Lemma SRPC_M_net_in_net_R_in_lock [N : MNet] [ n s v MQ M S] :
+      net_sane N ->
       NetMod.get n N = mserv MQ M S ->
       List.In (TrRecv (s, R) v) MQ ->
       exists c, SRPC_serv (Lock c s) (NetMod.get n N).
@@ -263,8 +262,8 @@ Module Type SOUND_F(Import Conf : DETECT_CONF)(Import Params : DETECT_PARAMS(Con
       consider (exists c, srpc = Lock c s); eattac.
     Qed.
 
-    Lemma SRPC_M_net_in_net_Q_out_lock [N n s v MQ M S] :
-      net_sane '' N ->
+    Lemma SRPC_M_net_in_net_Q_out_lock [N : MNet] [ n s v MQ M S] :
+      net_sane N ->
       NetMod.get n N = mserv MQ M S ->
       List.In (TrSend (s, Q) v) MQ ->
       exists c, SRPC_serv (Lock c s) (NetMod.get n N).
@@ -275,8 +274,8 @@ Module Type SOUND_F(Import Conf : DETECT_CONF)(Import Params : DETECT_PARAMS(Con
       consider (exists c, srpc = Lock c s); eattac.
     Qed.
 
-    Lemma SRPC_M_net_in_net_Q_out_uniq_M [N n c v v' MQ0 MQ1 M I P O] :
-      net_sane '' N ->
+    Lemma SRPC_M_net_in_net_Q_out_uniq_M [N : MNet] [ n c v v' MQ0 MQ1 M I P O] :
+      net_sane N ->
       NetMod.get n N = mserv (MQ0 ++ TrSend (c, R) v :: MQ1) M (serv I P O) ->
       ~ List.In (c, R, v') (MQ_s (MQ0 ++ MQ1) ++ O).
 
@@ -298,8 +297,8 @@ Module Type SOUND_F(Import Conf : DETECT_CONF)(Import Params : DETECT_PARAMS(Con
         bs (~ List.In (c, R, v) (O0 ++ O1)).
     Qed.
 
-    Lemma SRPC_M_net_in_net_Q_out_uniq_M0 [N n c v v' MQ0 MQ1 M S] :
-      net_sane '' N ->
+    Lemma SRPC_M_net_in_net_Q_out_uniq_M0 [N : MNet] [ n c v v' MQ0 MQ1 M S] :
+      net_sane N ->
       NetMod.get n N = mserv (MQ0 ++ TrSend (c, R) v :: MQ1) M S ->
       ~ List.In (TrSend (c, R) v') MQ0.
     Proof.
@@ -307,8 +306,8 @@ Module Type SOUND_F(Import Conf : DETECT_CONF)(Import Params : DETECT_PARAMS(Con
       assert (~ List.In (c, R, v') (MQ_s (MQ0 ++ MQ1) ++ &O)) by eauto using SRPC_M_net_in_net_Q_out_uniq_M.
       attac.
     Qed.
-    Lemma SRPC_M_net_in_net_Q_out_uniq_M1 [N n c v v' MQ0 MQ1 M S] :
-      net_sane '' N ->
+    Lemma SRPC_M_net_in_net_Q_out_uniq_M1 [N : MNet] [ n c v v' MQ0 MQ1 M S] :
+      net_sane N ->
       NetMod.get n N = mserv (MQ0 ++ TrSend (c, R) v :: MQ1) M S ->
       ~ List.In (TrSend (c, R) v') MQ1.
     Proof.
@@ -316,8 +315,8 @@ Module Type SOUND_F(Import Conf : DETECT_CONF)(Import Params : DETECT_PARAMS(Con
       assert (~ List.In (c, R, v') (MQ_s (MQ0 ++ MQ1) ++ &O)) by eauto using SRPC_M_net_in_net_Q_out_uniq_M.
       attac.
     Qed.
-    Lemma SRPC_M_net_in_net_Q_out_uniq_MP [N n c v v' MQ0 MQ1 M I P O] :
-      net_sane '' N ->
+    Lemma SRPC_M_net_in_net_Q_out_uniq_MP [N : MNet] [ n c v v' MQ0 MQ1 M I P O] :
+      net_sane N ->
       NetMod.get n N = mserv (MQ0 ++ TrSend (c, R) v :: MQ1) M (serv I P O) ->
       ~ List.In (c, R, v') O.
     Proof.
@@ -326,8 +325,8 @@ Module Type SOUND_F(Import Conf : DETECT_CONF)(Import Params : DETECT_PARAMS(Con
       attac.
     Qed.
 
-    Lemma SRPC_M_net_in_net_Q_out_uniq_P [N n c v v' MQ M I P O O'] :
-      net_sane '' N ->
+    Lemma SRPC_M_net_in_net_Q_out_uniq_P [N : MNet] [ n c v v' MQ M I P O O'] :
+      net_sane N ->
       NetMod.get n N = mserv MQ M (serv I P O) ->
       Deq (c, R) v O O' ->
       ~ (List.In (c, R, v') (MQ_s MQ ++ O')).
@@ -347,8 +346,8 @@ Module Type SOUND_F(Import Conf : DETECT_CONF)(Import Params : DETECT_PARAMS(Con
         bs (~ List.In (c, R, v) (O1 ++ O')).
     Qed.
 
-    Lemma SRPC_M_net_in_net_Q_out_uniq_PM [N n c v v' MQ M I P O O'] :
-      net_sane '' N ->
+    Lemma SRPC_M_net_in_net_Q_out_uniq_PM [N : MNet] [ n c v v' MQ M I P O O'] :
+      net_sane N ->
       NetMod.get n N = mserv MQ M (serv I P O) ->
       Deq (c, R) v O O' ->
       ~ (List.In (TrSend (c, R) v') MQ).
@@ -357,8 +356,8 @@ Module Type SOUND_F(Import Conf : DETECT_CONF)(Import Params : DETECT_PARAMS(Con
       assert (~ (List.In (c, R, v') (MQ_s MQ ++ O'))) by eauto using SRPC_M_net_in_net_Q_out_uniq_P.
       attac.
     Qed.
-    Lemma SRPC_M_net_in_net_Q_out_uniq_PP [N n c v v' MQ M I P O O'] :
-      net_sane '' N ->
+    Lemma SRPC_M_net_in_net_Q_out_uniq_PP [N : MNet] [ n c v v' MQ M I P O O'] :
+      net_sane N ->
       NetMod.get n N = mserv MQ M (serv I P O) ->
       Deq (c, R) v O O' ->
       ~ (List.In (c, R, v') O').
@@ -368,8 +367,8 @@ Module Type SOUND_F(Import Conf : DETECT_CONF)(Import Params : DETECT_PARAMS(Con
       attac.
     Qed.
 
-    Lemma SRPC_M_net_in_net_R_Q_M [N n s v v' MQ M I P O] :
-      net_sane '' N ->
+    Lemma SRPC_M_net_in_net_R_Q_M [N : MNet] [ n s v v' MQ M I P O] :
+      net_sane N ->
       NetMod.get n N = mserv MQ M (serv I P O) ->
       List.In (TrRecv (s, R) v) MQ ->
       ~ (List.In (s, Q, v') (MQ_s MQ ++ O)).
@@ -378,8 +377,8 @@ Module Type SOUND_F(Import Conf : DETECT_CONF)(Import Params : DETECT_PARAMS(Con
       unfold net_deinstr, deinstr in *; hsimpl in *.
       attac.
     Qed.
-    Lemma SRPC_M_net_in_net_R_Q_MM [N n s v v' MQ M S] :
-      net_sane '' N ->
+    Lemma SRPC_M_net_in_net_R_Q_MM [N : MNet] [ n s v v' MQ M S] :
+      net_sane N ->
       NetMod.get n N = mserv MQ M S ->
       List.In (TrRecv (s, R) v) MQ ->
       ~ (List.In (TrSend (s, Q) v') MQ).
@@ -388,8 +387,8 @@ Module Type SOUND_F(Import Conf : DETECT_CONF)(Import Params : DETECT_PARAMS(Con
       assert ( ~ (List.In (s, Q, v') (MQ_s MQ ++ &O))) by eauto using SRPC_M_net_in_net_R_Q_M.
       attac.
     Qed.
-    Lemma SRPC_M_net_in_net_R_Q_MP [N n s v v' MQ M I P O] :
-      net_sane '' N ->
+    Lemma SRPC_M_net_in_net_R_Q_MP [N : MNet] [ n s v v' MQ M I P O] :
+      net_sane N ->
       NetMod.get n N = mserv MQ M (serv I P O) ->
       List.In (TrRecv (s, R) v) MQ ->
       ~ (List.In (TrSend (s, Q) v') MQ).
@@ -399,8 +398,8 @@ Module Type SOUND_F(Import Conf : DETECT_CONF)(Import Params : DETECT_PARAMS(Con
       attac.
     Qed.
 
-    Lemma SRPC_M_net_in_net_R_Q_P [N n s v v' MQ M I P O] :
-      net_sane '' N ->
+    Lemma SRPC_M_net_in_net_R_Q_P [N : MNet] [ n s v v' MQ M I P O] :
+      net_sane N ->
       NetMod.get n N = mserv MQ M (serv I P O) ->
       List.In (s, R, v) I ->
       ~ (List.In (s, Q, v') (MQ_s MQ ++ O)).
@@ -409,8 +408,8 @@ Module Type SOUND_F(Import Conf : DETECT_CONF)(Import Params : DETECT_PARAMS(Con
       unfold net_deinstr, deinstr in *; hsimpl in *.
       attac.
     Qed.
-    Lemma SRPC_M_net_in_net_R_Q_PM [N n s v v' MQ M I P O] :
-      net_sane '' N ->
+    Lemma SRPC_M_net_in_net_R_Q_PM [N : MNet] [ n s v v' MQ M I P O] :
+      net_sane N ->
       NetMod.get n N = mserv MQ M (serv I P O) ->
       List.In (s, R, v) I ->
       ~ (List.In (TrSend (s, Q) v') MQ).
@@ -419,8 +418,8 @@ Module Type SOUND_F(Import Conf : DETECT_CONF)(Import Params : DETECT_PARAMS(Con
       assert ( ~ (List.In (s, Q, v') (MQ_s MQ ++ &O))) by eauto using SRPC_M_net_in_net_R_Q_P.
       attac.
     Qed.
-    Lemma SRPC_M_net_in_net_R_Q_PP [N n s v v' MQ M I P O] :
-      net_sane '' N ->
+    Lemma SRPC_M_net_in_net_R_Q_PP [N : MNet] [ n s v v' MQ M I P O] :
+      net_sane N ->
       NetMod.get n N = mserv MQ M (serv I P O) ->
       List.In (s, R, v) I ->
       ~ (List.In (s, Q, v') O).
@@ -430,8 +429,8 @@ Module Type SOUND_F(Import Conf : DETECT_CONF)(Import Params : DETECT_PARAMS(Con
       attac.
     Qed.
 
-    Lemma SRPC_M_net_in_net_Q_R_M [N n s v v' MQ M I P O] :
-      net_sane '' N ->
+    Lemma SRPC_M_net_in_net_Q_R_M [N : MNet] [ n s v v' MQ M I P O] :
+      net_sane N ->
       NetMod.get n N = mserv MQ M (serv I P O) ->
       List.In (TrSend (s, Q) v) MQ ->
       ~ (List.In (s, R, v') (I ++ MQ_r MQ)).
@@ -440,8 +439,8 @@ Module Type SOUND_F(Import Conf : DETECT_CONF)(Import Params : DETECT_PARAMS(Con
       unfold net_deinstr, deinstr in *; hsimpl in *.
       attac.
     Qed.
-    Lemma SRPC_M_net_in_net_Q_R_MM [N n s v v' MQ M S] :
-      net_sane '' N ->
+    Lemma SRPC_M_net_in_net_Q_R_MM [N : MNet] [ n s v v' MQ M S] :
+      net_sane N ->
       NetMod.get n N = mserv MQ M S ->
       List.In (TrSend (s, Q) v) MQ ->
       ~ (List.In (TrRecv (s, R) v') MQ).
@@ -450,8 +449,8 @@ Module Type SOUND_F(Import Conf : DETECT_CONF)(Import Params : DETECT_PARAMS(Con
       assert ( ~ (List.In (s, R, v') (&I ++ MQ_r MQ))) by eauto using SRPC_M_net_in_net_Q_R_M.
       attac.
     Qed.
-    Lemma SRPC_M_net_in_net_Q_R_MP [N n s v v' MQ M I P O] :
-      net_sane '' N ->
+    Lemma SRPC_M_net_in_net_Q_R_MP [N : MNet] [ n s v v' MQ M I P O] :
+      net_sane N ->
       NetMod.get n N = mserv MQ M (serv I P O) ->
       List.In (TrSend (s, Q) v) MQ ->
       ~ (List.In (s, R, v') I).
@@ -461,8 +460,8 @@ Module Type SOUND_F(Import Conf : DETECT_CONF)(Import Params : DETECT_PARAMS(Con
       attac.
     Qed.
 
-    Lemma SRPC_M_net_in_net_Q_R_P [N n s v v' MQ M I P O] :
-      net_sane '' N ->
+    Lemma SRPC_M_net_in_net_Q_R_P [N : MNet] [ n s v v' MQ M I P O] :
+      net_sane N ->
       NetMod.get n N = mserv MQ M (serv I P O) ->
       List.In (s, Q, v) O ->
       ~ (List.In (s, R, v') (I ++ MQ_r MQ)).
@@ -471,8 +470,8 @@ Module Type SOUND_F(Import Conf : DETECT_CONF)(Import Params : DETECT_PARAMS(Con
       unfold net_deinstr, deinstr in *; hsimpl in *.
       attac.
     Qed.
-    Lemma SRPC_M_net_in_net_Q_R_PM [N n s v v' MQ M I P O] :
-      net_sane '' N ->
+    Lemma SRPC_M_net_in_net_Q_R_PM [N : MNet] [ n s v v' MQ M I P O] :
+      net_sane N ->
       NetMod.get n N = mserv MQ M (serv I P O) ->
       List.In (s, Q, v) O ->
       ~ (List.In (TrRecv (s, R) v') MQ).
@@ -481,8 +480,8 @@ Module Type SOUND_F(Import Conf : DETECT_CONF)(Import Params : DETECT_PARAMS(Con
       assert ( ~ (List.In (s, R, v') (&I ++ MQ_r MQ))) by eauto using SRPC_M_net_in_net_Q_R_P.
       attac.
     Qed.
-    Lemma SRPC_M_net_in_net_Q_R_PP [N n s v v' MQ M I P O] :
-      net_sane '' N ->
+    Lemma SRPC_M_net_in_net_Q_R_PP [N : MNet] [ n s v v' MQ M I P O] :
+      net_sane N ->
       NetMod.get n N = mserv MQ M (serv I P O) ->
       List.In (s, Q, v) O ->
       ~ (List.In (s, R, v') I).
@@ -492,8 +491,8 @@ Module Type SOUND_F(Import Conf : DETECT_CONF)(Import Params : DETECT_PARAMS(Con
       attac.
     Qed.
 
-    Lemma SRPC_M_net_in_net_Q_excl_R_M [N n c v v' MQ M I P O] :
-      net_sane '' N ->
+    Lemma SRPC_M_net_in_net_Q_excl_R_M [N : MNet] [ n c v v' MQ M I P O] :
+      net_sane N ->
       NetMod.get n N = mserv MQ M (serv I P O) ->
       List.In (TrRecv (c, Q) v) MQ ->
       ~ List.In (c, R, v') (MQ_s MQ ++ O).
@@ -502,8 +501,8 @@ Module Type SOUND_F(Import Conf : DETECT_CONF)(Import Params : DETECT_PARAMS(Con
       unfold net_deinstr, deinstr in *; hsimpl in *.
       attac.
     Qed.
-    Lemma SRPC_M_net_in_net_Q_excl_R_MM [N n c v v' MQ M S] :
-      net_sane '' N ->
+    Lemma SRPC_M_net_in_net_Q_excl_R_MM [N : MNet] [ n c v v' MQ M S] :
+      net_sane N ->
       NetMod.get n N = mserv MQ M S ->
       List.In (TrRecv (c, Q) v) MQ ->
       ~ List.In (TrSend (c, R) v') MQ.
@@ -512,8 +511,8 @@ Module Type SOUND_F(Import Conf : DETECT_CONF)(Import Params : DETECT_PARAMS(Con
       assert (~ List.In (c, R, v') (MQ_s MQ ++ &O)) by eauto using SRPC_M_net_in_net_Q_excl_R_M.
       attac.
     Qed.
-    Lemma SRPC_M_net_in_net_Q_excl_R_MP [N n c v v' MQ M I P O] :
-      net_sane '' N ->
+    Lemma SRPC_M_net_in_net_Q_excl_R_MP [N : MNet] [ n c v v' MQ M I P O] :
+      net_sane N ->
       NetMod.get n N = mserv MQ M (serv I P O) ->
       List.In (TrRecv (c, Q) v) MQ ->
       ~ List.In (c, R, v') O.
@@ -523,8 +522,8 @@ Module Type SOUND_F(Import Conf : DETECT_CONF)(Import Params : DETECT_PARAMS(Con
       attac.
     Qed.
 
-    Lemma SRPC_M_net_in_net_Q_excl_R_P [N n c v v' MQ M I P O] :
-      net_sane '' N ->
+    Lemma SRPC_M_net_in_net_Q_excl_R_P [N : MNet] [ n c v v' MQ M I P O] :
+      net_sane N ->
       NetMod.get n N = mserv MQ M (serv I P O) ->
       List.In (c, Q, v) I ->
       ~ List.In (c, R, v') (MQ_s MQ ++ O).
@@ -533,8 +532,8 @@ Module Type SOUND_F(Import Conf : DETECT_CONF)(Import Params : DETECT_PARAMS(Con
       unfold net_deinstr, deinstr in *; hsimpl in *.
       attac.
     Qed.
-    Lemma SRPC_M_net_in_net_Q_excl_R_PM [N n c v v' MQ M I P O] :
-      net_sane '' N ->
+    Lemma SRPC_M_net_in_net_Q_excl_R_PM [N : MNet] [ n c v v' MQ M I P O] :
+      net_sane N ->
       NetMod.get n N = mserv MQ M (serv I P O) ->
       List.In (c, Q, v) I ->
       ~ List.In (TrSend (c, R) v') MQ.
@@ -543,8 +542,8 @@ Module Type SOUND_F(Import Conf : DETECT_CONF)(Import Params : DETECT_PARAMS(Con
       assert (~ List.In (c, R, v') (MQ_s MQ ++ &O)) by eauto using SRPC_M_net_in_net_Q_excl_R_P.
       attac.
     Qed.
-    Lemma SRPC_M_net_in_net_Q_excl_R_PP [N n c v v' MQ M I P O] :
-      net_sane '' N ->
+    Lemma SRPC_M_net_in_net_Q_excl_R_PP [N : MNet] [ n c v v' MQ M I P O] :
+      net_sane N ->
       NetMod.get n N = mserv MQ M (serv I P O) ->
       List.In (c, Q, v) I ->
       ~ List.In (c, R, v') O.
@@ -554,8 +553,8 @@ Module Type SOUND_F(Import Conf : DETECT_CONF)(Import Params : DETECT_PARAMS(Con
       attac.
     Qed.
 
-    Lemma SRPC_M_net_in_net_Q_excl_c_M [N n c v MQ M I P O] :
-      net_sane '' N ->
+    Lemma SRPC_M_net_in_net_Q_excl_c_M [N : MNet] [ n c v MQ M I P O] :
+      net_sane N ->
       NetMod.get n N = mserv MQ M (serv I P O) ->
       List.In (TrRecv (c, Q) v) MQ ->
       ~ proc_client c P.
@@ -565,8 +564,8 @@ Module Type SOUND_F(Import Conf : DETECT_CONF)(Import Params : DETECT_PARAMS(Con
       attac.
     Qed.
 
-    Lemma SRPC_M_net_in_net_Q_excl_c_P [N n c v MQ M I P O] :
-      net_sane '' N ->
+    Lemma SRPC_M_net_in_net_Q_excl_c_P [N : MNet] [ n c v MQ M I P O] :
+      net_sane N ->
       NetMod.get n N = mserv MQ M (serv I P O) ->
       List.In (c, Q, v) I ->
       ~ proc_client c P.
@@ -576,8 +575,8 @@ Module Type SOUND_F(Import Conf : DETECT_CONF)(Import Params : DETECT_PARAMS(Con
       attac.
     Qed.
 
-    Lemma SRPC_M_net_in_net_R_excl_Q_M [N n c v v' MQ M I P O] :
-      net_sane '' N ->
+    Lemma SRPC_M_net_in_net_R_excl_Q_M [N : MNet] [ n c v v' MQ M I P O] :
+      net_sane N ->
       NetMod.get n N = mserv MQ M (serv I P O) ->
       List.In (TrSend (c, R) v) MQ ->
       ~ List.In (c, Q, v') (I ++ MQ_r MQ).
@@ -586,8 +585,8 @@ Module Type SOUND_F(Import Conf : DETECT_CONF)(Import Params : DETECT_PARAMS(Con
       unfold net_deinstr, deinstr in *; hsimpl in *.
       attac.
     Qed.
-    Lemma SRPC_M_net_in_net_R_excl_Q_MM [N n c v v' MQ M S] :
-      net_sane '' N ->
+    Lemma SRPC_M_net_in_net_R_excl_Q_MM [N : MNet] [ n c v v' MQ M S] :
+      net_sane N ->
       NetMod.get n N = mserv MQ M S ->
       List.In (TrSend (c, R) v) MQ ->
       ~ List.In (TrRecv (c, Q) v') MQ.
@@ -596,8 +595,8 @@ Module Type SOUND_F(Import Conf : DETECT_CONF)(Import Params : DETECT_PARAMS(Con
       assert (~ List.In (c, Q, v') (&I ++ MQ_r MQ)) by eauto using SRPC_M_net_in_net_R_excl_Q_M.
       attac.
     Qed.
-    Lemma SRPC_M_net_in_net_R_excl_Q_MP [N n c v v' MQ M I P O] :
-      net_sane '' N ->
+    Lemma SRPC_M_net_in_net_R_excl_Q_MP [N : MNet] [ n c v v' MQ M I P O] :
+      net_sane N ->
       NetMod.get n N = mserv MQ M (serv I P O) ->
       List.In (TrSend (c, R) v) MQ ->
       ~ List.In (c, Q, v') I.
@@ -607,8 +606,8 @@ Module Type SOUND_F(Import Conf : DETECT_CONF)(Import Params : DETECT_PARAMS(Con
       attac.
     Qed.
 
-    Lemma SRPC_M_net_in_net_R_excl_Q_P [N n c v v' MQ M I P O] :
-      net_sane '' N ->
+    Lemma SRPC_M_net_in_net_R_excl_Q_P [N : MNet] [ n c v v' MQ M I P O] :
+      net_sane N ->
       NetMod.get n N = mserv MQ M (serv I P O) ->
       List.In (c, R, v) O ->
       ~ List.In (c, Q, v') (I ++ MQ_r MQ).
@@ -617,8 +616,8 @@ Module Type SOUND_F(Import Conf : DETECT_CONF)(Import Params : DETECT_PARAMS(Con
       unfold net_deinstr, deinstr in *; hsimpl in *.
       attac.
     Qed.
-    Lemma SRPC_M_net_in_net_R_excl_Q_PM [N n c v v' MQ M I P O] :
-      net_sane '' N ->
+    Lemma SRPC_M_net_in_net_R_excl_Q_PM [N : MNet] [ n c v v' MQ M I P O] :
+      net_sane N ->
       NetMod.get n N = mserv MQ M (serv I P O) ->
       List.In (c, R, v) O ->
       ~ List.In (TrRecv (c, Q) v') MQ.
@@ -627,8 +626,8 @@ Module Type SOUND_F(Import Conf : DETECT_CONF)(Import Params : DETECT_PARAMS(Con
       assert (~ List.In (c, Q, v') (&I ++ MQ_r MQ)) by eauto using SRPC_M_net_in_net_R_excl_Q_P.
       attac.
     Qed.
-    Lemma SRPC_M_net_in_net_R_excl_Q_PP [N n c v v' MQ M I P O] :
-      net_sane '' N ->
+    Lemma SRPC_M_net_in_net_R_excl_Q_PP [N : MNet] [ n c v v' MQ M I P O] :
+      net_sane N ->
       NetMod.get n N = mserv MQ M (serv I P O) ->
       List.In (c, R, v) O ->
       ~ List.In (c, Q, v') I.
@@ -638,8 +637,8 @@ Module Type SOUND_F(Import Conf : DETECT_CONF)(Import Params : DETECT_PARAMS(Con
       attac.
     Qed.
 
-    Lemma SRPC_M_net_in_net_R_excl_c_M [N n c v MQ M I P O] :
-      net_sane '' N ->
+    Lemma SRPC_M_net_in_net_R_excl_c_M [N : MNet] [ n c v MQ M I P O] :
+      net_sane N ->
       NetMod.get n N = mserv MQ M (serv I P O) ->
       List.In (TrRecv (c, Q) v) MQ ->
       ~ proc_client c P.
@@ -649,8 +648,8 @@ Module Type SOUND_F(Import Conf : DETECT_CONF)(Import Params : DETECT_PARAMS(Con
       attac.
     Qed.
 
-    Lemma SRPC_M_net_in_net_R_excl_c_P [N n c v MQ M I P O] :
-      net_sane '' N ->
+    Lemma SRPC_M_net_in_net_R_excl_c_P [N : MNet] [ n c v MQ M I P O] :
+      net_sane N ->
       NetMod.get n N = mserv MQ M (serv I P O) ->
       List.In (c, Q, v) I ->
       ~ proc_client c P.
@@ -660,8 +659,8 @@ Module Type SOUND_F(Import Conf : DETECT_CONF)(Import Params : DETECT_PARAMS(Con
       attac.
     Qed.
 
-    Lemma SRPC_M_net_in_net_c_excl_Q_M [N n c v MQ M I P O] :
-      net_sane '' N ->
+    Lemma SRPC_M_net_in_net_c_excl_Q_M [N : MNet] [ n c v MQ M I P O] :
+      net_sane N ->
       NetMod.get n N = mserv MQ M (serv I P O) ->
       proc_client c P ->
       ~ List.In (TrRecv (c, Q) v) MQ.
@@ -672,8 +671,8 @@ Module Type SOUND_F(Import Conf : DETECT_CONF)(Import Params : DETECT_PARAMS(Con
       eattac.
     Qed.
 
-    Lemma SRPC_M_net_in_net_c_excl_Q_P [N n c v MQ M I P O] :
-      net_sane '' N ->
+    Lemma SRPC_M_net_in_net_c_excl_Q_P [N : MNet] [ n c v MQ M I P O] :
+      net_sane N ->
       NetMod.get n N = mserv MQ M (serv I P O) ->
       proc_client c P ->
       ~ List.In (c, Q, v) (I).
@@ -684,8 +683,8 @@ Module Type SOUND_F(Import Conf : DETECT_CONF)(Import Params : DETECT_PARAMS(Con
       iattac.
     Qed.
 
-    Lemma SRPC_M_net_in_net_c_excl_R [N n c v MQ M I P O] :
-      net_sane '' N ->
+    Lemma SRPC_M_net_in_net_c_excl_R [N : MNet] [ n c v MQ M I P O] :
+      net_sane N ->
       NetMod.get n N = mserv MQ M (serv I P O) ->
       proc_client c P ->
       ~ List.In (c, R, v) (MQ_s MQ ++ O).
@@ -695,8 +694,8 @@ Module Type SOUND_F(Import Conf : DETECT_CONF)(Import Params : DETECT_PARAMS(Con
       iattac.
     Qed.
 
-    Lemma SRPC_M_net_in_net_c_excl_R_M [N n c v MQ M I P O] :
-      net_sane '' N ->
+    Lemma SRPC_M_net_in_net_c_excl_R_M [N : MNet] [ n c v MQ M I P O] :
+      net_sane N ->
       NetMod.get n N = mserv MQ M (serv I P O) ->
       proc_client c P ->
       ~ List.In (TrSend (c, R) v) MQ.
@@ -706,8 +705,8 @@ Module Type SOUND_F(Import Conf : DETECT_CONF)(Import Params : DETECT_PARAMS(Con
       iattac.
     Qed.
 
-    Lemma SRPC_M_net_in_net_c_excl_R_P [N n c v MQ M I P O] :
-      net_sane '' N ->
+    Lemma SRPC_M_net_in_net_c_excl_R_P [N : MNet] [ n c v MQ M I P O] :
+      net_sane N ->
       NetMod.get n N = mserv MQ M (serv I P O) ->
       proc_client c P ->
       ~ List.In (c, R, v) O.
@@ -777,7 +776,7 @@ Module Type SOUND_F(Import Conf : DETECT_CONF)(Import Params : DETECT_PARAMS(Con
   #[export] Hint Constructors sends_to_mon : LTS.
 
 
-  Definition sends_to N n0 n1 p := sends_to_mon (get_Mc N n0) n1 p.
+  Definition sends_to (N : MNet) n0 n1 p := sends_to_mon (mserv_m (N n0)) n1 p.
   #[export] Hint Unfold sends_to : LTS_get.
   #[export] Hint Transparent sends_to : LTS.
 
@@ -800,7 +799,7 @@ Module Type SOUND_F(Import Conf : DETECT_CONF)(Import Params : DETECT_PARAMS(Con
   Qed.
 
 
-  Lemma sends_to_dec MN0 n0 n1 p : (sends_to MN0 n0 n1 p \/ ~ sends_to MN0 n0 n1 p).
+  Lemma sends_to_dec (MN0 : MNet) n0 n1 p : (sends_to MN0 n0 n1 p \/ ~ sends_to MN0 n0 n1 p).
 
   Proof.
     unfold sends_to.
@@ -821,8 +820,6 @@ Module Type SOUND_F(Import Conf : DETECT_CONF)(Import Params : DETECT_PARAMS(Con
     sends_to_mon (MSend nc p1 (MRecv state)) n p0 <->
       nc = (n, R) /\ p1 = p0.
   Proof. destruct nc as [n' [|]]; split; attac; try (kill H); attac. Qed.
-
-  Import Rad.
 
   Lemma sends_to_mon_many_inv state n ns t p0 p1 :
     sends_to_mon (MSend_all ns t p1 (MRecv state)) n p0 <->
@@ -853,237 +850,165 @@ Module Type SOUND_F(Import Conf : DETECT_CONF)(Import Params : DETECT_PARAMS(Con
     | MSend (_, t) _ m' => t = R /\ no_Q_probe m'
     end.
 
-  Definition no_Q_probe_in MN n := no_Q_probe (get_Mc MN n).
+  Definition no_Q_probe_in (MN : MNet) n := no_Q_probe (mserv_m (MN n)).
 
 
   Inductive KIS (MN : MNet) :=
     KIS_
       (* We are sane *)
-      (H_sane_S : net_sane '' MN)
+      (H_sane_S : net_sane MN)
       (* `self` is correct *)
-      (H_self_S : forall n0, _of self MN n0 = n0)
-      (* We are using the algorithm *)
-      (H_Rad_S : forall n0, handle (get_M MN n0) = Rad.Rad_handle)
+      (H_self_S : forall n0, self (MN n0) = n0)
       (* Monitor correctly judges the lock, unless there is a reply incoming it is about to see *)
-      (H_lock_S : forall n0 n1, _of lock MN n0 = Some n1 -> net_lock_on '' MN n0 n1 \/ exists v, List.In (TrRecv (n1, R) v) (get_MQ MN n0))
+      (H_lock_S : forall n0 n1, lock (MN n0) = Some n1 -> net_lock_on MN n0 n1 \/ exists v, List.In (TrRecv (n1, R) v) (mserv_i (MN n0)))
       (* All members of the waiting list are locked on us *)
-      (H_wait_S : forall n0 n1, List.In n0 (_of waitees MN n1) -> net_lock_on '' MN n0 n1)
+      (H_wait_S : forall n0 n1, List.In n0 (wait (MN n1)) -> net_lock_on MN n0 n1)
       (* Monitors send probes only to those locked. *)
-      (H_sendp_S : forall n0 n1 p, sends_to MN n1 n0 p -> net_lock_on '' MN n0 n1)
+      (H_sendp_S : forall n0 n1 p, sends_to MN n1 n0 p -> net_lock_on MN n0 n1)
       (* All sent probes have their index no higher than the lock id of the initiator *)
-      (H_index_send_S : forall n0 n1 p, sends_to MN n0 n1 p -> (index p <= _of lock_id MN (init p))%nat)
-      (* All received probes have their index no higher than the lock id of the initiator *)
-      (H_index_recvp_S : forall n0 n1 p, List.In (EvRecv (n1, R) p) (get_MQ MN n0) -> (index p <= _of lock_id MN (init p))%nat)
-      (* If we are about to receive a hot probe of someone whose monitor considers locked, then we depend on them. *)
-      (H_sendp_hot_S : forall n0 n1 n2, sends_to MN n1 n0 (hot_of MN n2) -> _of lock MN n2 <> None -> dep_on '' MN n0 n2)
+      (H_sendp_hot_S : forall n0 n1 n2, sends_to MN n1 n0 (hot_of n2) -> lock (MN n2) <> None -> dep_on MN n0 n2)
       (* If we received a hot probe of someone whose monitor considers locked, then we depend on them. *)
-      (H_recvp_hot_S : forall n0 n1 n2, List.In (hot_ev_of MN n2 n0) (get_MQ MN n1) -> _of lock MN n0 <> None -> dep_on '' MN n1 n0)
+      (H_recvp_hot_S : forall n0 n1 n2, List.In (hot_ev_of n2 n0) (mserv_i (MN n1)) -> lock (MN n0) <> None -> dep_on MN n1 n0)
       (* No false alarms: if anyone screams, they are indeed deadlocked *)
-      (H_alarm_S : forall n, _of alarm MN n = true -> dep_on '' MN n n)
+      (H_alarm_S : forall n, alarm (MN n) = true -> dep_on MN n n)
       : KIS MN.
 
 
-  Lemma KIS_sane [MN] : KIS MN -> net_sane '' MN.
+  Lemma KIS_sane [MN] : KIS MN -> net_sane MN.
   Proof. intros; consider (KIS _). Qed.
 
-  Lemma KIS_self [MN] : KIS MN -> forall n0, _of self MN n0 = n0.
+  Lemma KIS_self [MN] : KIS MN -> forall n0, self (MN n0) = n0.
   Proof. intros; consider (KIS _). Qed.
 
-  Lemma KIS_Rad [MN] : KIS MN -> forall n0, handle (get_M MN n0) = Rad.Rad_handle.
+  Lemma KIS_lock [MN] : KIS MN -> forall n0 n1, lock (MN n0) = Some n1 -> net_lock_on MN n0 n1 \/ exists v, List.In (TrRecv (n1, R) v) (mserv_i (MN n0)).
   Proof. intros; consider (KIS _). Qed.
 
-  Lemma KIS_lock [MN] : KIS MN -> forall n0 n1, _of lock MN n0 = Some n1 -> net_lock_on '' MN n0 n1 \/ exists v, List.In (TrRecv (n1, R) v) (get_MQ MN n0).
+  Lemma KIS_wait [MN] : KIS MN -> forall n0 n1, List.In n0 (wait (MN n1)) -> net_lock_on MN n0 n1.
   Proof. intros; consider (KIS _). Qed.
 
-  Lemma KIS_wait [MN] : KIS MN -> forall n0 n1, List.In n0 (_of waitees MN n1) -> net_lock_on '' MN n0 n1.
-  Proof. intros; consider (KIS _). Qed.
-
-  Lemma KIS_sendp [MN] : KIS MN -> forall n0 n1 p, sends_to MN n1 n0 p -> net_lock_on '' MN n0 n1.
+  Lemma KIS_sendp [MN] : KIS MN -> forall n0 n1 p, sends_to MN n1 n0 p -> net_lock_on MN n0 n1.
   Proof. intros; consider (KIS _). eauto. Qed.
 
-  Lemma KIS_index_sendp [MN] : KIS MN -> forall n0 n1 p, sends_to MN n0 n1 p -> (index p <= _of lock_id MN (init p))%nat.
+  Lemma KIS_sendp_hot [MN] : KIS MN -> forall n0 n1 n2, sends_to MN n1 n0 (hot_of n2) -> lock (MN n2) <> None -> dep_on MN n0 n2.
   Proof. intros; consider (KIS _). eauto. Qed.
 
-  Lemma KIS_index_recvp [MN] : KIS MN -> forall n0 n1 p, List.In (EvRecv (n1, R) p) (get_MQ MN n0) -> (index p <= _of lock_id MN (init p))%nat.
+  Lemma KIS_recvp_hot [MN] : KIS MN -> forall n0 n1 n2, List.In (hot_ev_of n2 n0 ) (mserv_i (MN n1)) -> lock (MN n0) <> None -> dep_on MN n1 n0.
   Proof. intros; consider (KIS _). eauto. Qed.
 
-  Lemma KIS_sendp_hot [MN] : KIS MN -> forall n0 n1 n2, sends_to MN n1 n0 (hot_of MN n2) -> _of lock MN n2 <> None -> dep_on '' MN n0 n2.
-  Proof. intros; consider (KIS _). eauto. Qed.
-
-  Lemma KIS_recvp_hot [MN] : KIS MN -> forall n0 n1 n2, List.In (hot_ev_of MN n2 n0) (get_MQ MN n1) -> _of lock MN n0 <> None -> dep_on '' MN n1 n0.
-  Proof. intros; consider (KIS _). eauto. Qed.
-
-  Lemma KIS_alarm [MN] : KIS MN -> forall n, _of alarm MN n = true -> dep_on '' MN n n.
+  Lemma KIS_alarm [MN] : KIS MN -> forall n, alarm (MN n) = true -> dep_on MN n n.
   Proof. intros; consider (KIS _). Qed.
 
   #[export] Hint Immediate
     KIS_sane
     KIS_self
-    KIS_Rad
     KIS_lock
     KIS_wait
     KIS_sendp
-    KIS_index_sendp
-    KIS_index_recvp
     KIS_sendp_hot
     KIS_recvp_hot
     KIS_alarm : LTS.
 
 
-  Lemma KIS_self_get [MN n0] [MQ h s S] [self'] :
+  Lemma KIS_self_get [MN n0] [MQ s S] [self'] :
     KIS MN ->
-    NetMod.get n0 MN = mserv MQ {|handle:=h; state:=s|} S ->
+    NetMod.get n0 MN = mserv MQ (s) S ->
     self (next_state s) = self' ->
     self' = n0.
 
-  Proof. intros. assert (_of self MN n0 = n0) by eauto with LTS.
+  Proof. intros. assert (self (MN n0) = n0) by eauto with LTS.
          ltac1:(autounfold with LTS_get in * ); hsimpl in * |-; auto.
   Qed.
 
 
-  Lemma KIS_Rad_get [MN n0] [MQ h s S] :
+  Lemma KIS_lock_get [MN n0 n1] [MQ s S] :
     KIS MN ->
-    NetMod.get n0 MN = mserv MQ {|handle:=h; state:=s|} S ->
-    h = Rad_handle.
-
-  Proof. intros. assert (handle (get_M MN n0) = Rad_handle) by eauto with LTS.
-         ltac1:(autounfold with LTS_get in * ); hsimpl in * |-; auto.
-  Qed.
-
-
-  Lemma KIS_lock_get [MN n0 n1] [MQ h s S] :
-    KIS MN ->
-    NetMod.get n0 MN = mserv MQ {|handle:=h; state:=s|} S ->
+    NetMod.get n0 MN = mserv MQ (s) S ->
     lock (next_state s) = Some n1 ->
-    net_lock_on '' MN n0 n1 \/ exists v, List.In (TrRecv (n1, R) v) MQ.
+    net_lock_on MN n0 n1 \/ exists v, List.In (TrRecv (n1, R) v) MQ.
 
   Proof. intros.
-         assert (_of lock MN n0 = Some n1) by (ltac1:(autounfold with LTS_get in * ); attac).
-         assert (net_lock_on '' MN n0 n1 \/ exists v, List.In (TrRecv (n1, R) v) (get_MQ MN n0)) by attac.
+         assert (lock (MN n0) = Some n1) by (ltac1:(autounfold with LTS_get in * ); attac).
+         assert (net_lock_on MN n0 n1 \/ exists v, List.In (TrRecv (n1, R) v) (mserv_i (MN n0))) by attac.
          ltac1:(autounfold with LTS_get in * ); hsimpl in * |-; auto.
   Qed.
 
 
-  Lemma KIS_wait_get [MN n0 n1] [MQ h s S] :
+  Lemma KIS_wait_get [MN n0 n1] [MQ s S] :
     KIS MN ->
-    NetMod.get n1 MN = mserv MQ {|handle:=h; state:=s|} S ->
-    List.In n0 (waitees (next_state s)) ->
-    net_lock_on '' MN n0 n1.
+    NetMod.get n1 MN = mserv MQ (s) S ->
+    List.In n0 (wait (next_state s)) ->
+    net_lock_on MN n0 n1.
 
   Proof. intros.
-         assert (List.In n0 (_of waitees MN n1)) by (ltac1:(autounfold with LTS_get in * ); attac).
-         assert (net_lock_on '' MN n0 n1) by attac.
+         assert (List.In n0 (wait (MN n1))) by (ltac1:(autounfold with LTS_get in * ); attac).
+         assert (net_lock_on MN n0 n1) by attac.
          ltac1:(autounfold with LTS_get in * ); hsimpl in * |-; auto.
   Qed.
 
 
-  Lemma KIS_index_sendp_get [MN n0 n1 n2 p] [MQ0 MQ2 h0 h2 s0 s2 S0 S2] [index' lock_id'] :
+  Lemma KIS_sendp_hot_get [MN n0 n1 n2 p] [MQ1 MQ2 s1 s2 S1 S2] :
     KIS MN ->
-    NetMod.get n0 MN = mserv MQ0 {|handle:=h0; state:=s0|} S0 ->
-    NetMod.get n2 MN = mserv MQ2 {|handle:=h2; state:=s2|} S2 ->
-    sends_to_mon s0 n1 p ->
-    index p = index' ->
-    init p = n2 ->
-    lock_id (next_state s2) = lock_id' ->
-    index' <= lock_id'.
-
-  Proof. intros.
-         assert (sends_to MN n0 n1 p) by (ltac1:(autounfold with LTS_get in * ); attac).
-         assert (index p <= _of lock_id MN (init p)) by attac.
-         destruct p; simpl in *.
-         ltac1:(autounfold with LTS_get in * ); attac.
-         attac.
-  Qed.
-
-
-  Lemma KIS_index_recvp_get [MN n0 n1 n2 p] [MQ0 MQ2 h0 h2 s0 s2 S0 S2] [index' lock_id'] :
-    KIS MN ->
-    NetMod.get n0 MN = mserv MQ0 {|handle:=h0; state:=s0|} S0 ->
-    NetMod.get n2 MN = mserv MQ2 {|handle:=h2; state:=s2|} S2 ->
-    List.In (EvRecv (n1, R) p) MQ0 ->
-    index p = index' ->
-    init p = n2 ->
-    lock_id (next_state s2) = lock_id' ->
-    index' <= lock_id'.
-
-  Proof. intros.
-         assert (List.In (EvRecv (n1, R) p) (get_MQ MN n0)) by (ltac1:(autounfold with LTS_get in * ); attac).
-         assert (index p <= _of lock_id MN (init p)) by attac.
-         destruct p; simpl in *.
-         ltac1:(autounfold with LTS_get in * ); attac.
-         attac.
-  Qed.
-
-
-  Lemma KIS_sendp_hot_get [MN n0 n1 n2 p] [MQ1 MQ2 h1 h2 s1 s2 S1 S2] [lock_id'] :
-    KIS MN ->
-    NetMod.get n1 MN = mserv MQ1 {|handle:=h1; state:=s1|} S1 ->
-    NetMod.get n2 MN = mserv MQ2 {|handle:=h2; state:=s2|} S2 ->
+    NetMod.get n1 MN = mserv MQ1 (s1) S1 ->
+    NetMod.get n2 MN = mserv MQ2 (s2) S2 ->
     sends_to_mon s1 n0 p ->
-    index p = lock_id (next_state s2) ->
     init p = n2 ->
-    lock_id (next_state s2) = lock_id' ->
     lock (next_state s2) <> None ->
-    dep_on '' MN n0 n2.
+    dep_on MN n0 n2.
 
   Proof. intros.
          destruct p.
-         assert (sends_to MN n1 n0 (hot_of MN n2)) by (unfold hot_of in *; ltac1:(autounfold with LTS_get in * ); attac).
-         assert (_of lock MN n2 <> None) by (ltac1:(autounfold with LTS_get in * ); attac).
+         assert (sends_to MN n1 n0 (hot_of n2)) by (unfold hot_of in *; ltac1:(autounfold with LTS_get in * ); attac).
+         assert (lock (MN n2) <> None) by (ltac1:(autounfold with LTS_get in * ); attac).
          eauto with LTS.
   Qed.
 
 
-  Lemma KIS_recvp_hot_get [MN n0 n1 n2 p] [MQ0 MQ2 h0 h2 s0 s2 S0 S2] [lock_id'] :
+  Lemma KIS_recvp_hot_get [MN n0 n1 n2 p] [MQ0 MQ2 s0 s2 S0 S2] :
     KIS MN ->
-    NetMod.get n0 MN = mserv MQ0 {|handle:=h0; state:=s0|} S0 ->
-    NetMod.get n2 MN = mserv MQ2 {|handle:=h2; state:=s2|} S2 ->
+    NetMod.get n0 MN = mserv MQ0 (s0) S0 ->
+    NetMod.get n2 MN = mserv MQ2 (s2) S2 ->
     List.In (EvRecv (n1, R) p) MQ0 ->
-    index p = lock_id (next_state s2) ->
     init p = n2 ->
-    lock_id (next_state s2) = lock_id' ->
     lock (next_state s2) <> None ->
-    dep_on '' MN n0 n2.
+    dep_on MN n0 n2.
 
   Proof. intros.
          destruct p.
-         assert (List.In (hot_ev_of MN n1 n2) (get_MQ MN n0)) by (unfold hot_ev_of, hot_of in *; ltac1:(autounfold with LTS_get in * ); attac).
-         assert (_of lock MN n2 <> None) by (ltac1:(autounfold with LTS_get in * ); attac).
+         assert (List.In (hot_ev_of n1 n2 ) (mserv_i (MN n0))) by (unfold hot_ev_of, hot_of in *; ltac1:(autounfold with LTS_get in * ); attac).
+         assert (lock (MN n2) <> None) by (ltac1:(autounfold with LTS_get in * ); attac).
          eauto with LTS.
   Qed.
 
 
-  Lemma KIS_alarm_get [MN n0] [MQ h s S] :
+  Lemma KIS_alarm_get [MN n0] [MQ s S] :
     KIS MN ->
-    NetMod.get n0 MN = mserv MQ {|handle:=h; state:=s|} S ->
+    NetMod.get n0 MN = mserv MQ (s) S ->
     alarm (next_state s) = true ->
-    dep_on '' MN n0 n0.
+    dep_on MN n0 n0.
 
   Proof. intros.
-         enough (_of alarm MN n0 = true) by attac.
+         enough (alarm (MN n0) = true) by attac.
          ltac1:(autounfold with LTS_get in * ); attac.
   Qed.
 
   Hint Resolve
     KIS_self_get
-    KIS_Rad_get
     KIS_lock_get
     KIS_wait_get
-    KIS_index_sendp_get
-    KIS_index_recvp_get
     KIS_sendp_hot_get
     KIS_recvp_hot_get
     KIS_alarm : LTS.
 
+  Notation "'' N" := (net_deinstr N) (at level 20).
 
   Lemma KIS_invariant_sane [MN0 MN1 a] :
     (MN0 =(a)=> MN1) ->
     KIS MN0 ->
-    net_sane '' MN1.
+    net_sane MN1.
 
   Proof.
     intros.
-    assert (net_sane '' MN0) by eauto with LTS.
+    assert (net_sane MN0) by eauto with LTS.
     destruct (MNAct_to_PNAct a) eqn:?.
     - eauto using net_deinstr_act_do with LTS.
     - now replace ('' MN1) with ('' MN0) by eauto using net_deinstr_act_skip with LTS.
@@ -1095,40 +1020,27 @@ Module Type SOUND_F(Import Conf : DETECT_CONF)(Import Params : DETECT_PARAMS(Con
   Lemma KIS_invariant_self [MN0 MN1 a] :
     (MN0 =(a)=> MN1) ->
     KIS MN0 ->
-    forall n0, _of self MN1 n0 = n0.
+    forall n0, self (MN1 n0) = n0.
 
   Proof.
     intros.
-    assert (_of self MN0 n0 = n0) by attac.
-    enough (_of self MN0 n0 = _of self MN1 n0) by attac.
-    enough (handle (get_M MN0 n0) = Rad.Rad_handle) by eauto using net_preserve_self with LTS.
-    attac.
+    assert (self (MN0 n0) = n0) by attac.
+    enough (self (MN0 n0) = self (MN1 n0)) by attac.
+    eauto using net_preserve_self with LTS.
   Qed.
 
   Hint Immediate KIS_invariant_self : LTS.
 
 
-  Lemma KIS_invariant_Rad [MN0 MN1 a] :
-    (MN0 =(a)=> MN1) ->
-    KIS MN0 ->
-    forall n0, handle (get_M MN1 n0) = Rad.Rad_handle.
-
-  Proof.
-    intros.
-    enough (handle (get_M MN0 n0) = handle (get_M MN1 n0)) by attac.
-    eauto using net_preserve_handle.
-  Qed.
-
-  Hint Immediate KIS_invariant_Rad : LTS.
-
   Ltac2 Notation "destruct_mna" a(constr) :=
       destruct $a as [? [[[? [|]]|[? [|]]|]|[[? ?]|[? ?]|]|[[? ?]|[? ?]|]] | ? ? [|] [?|?]]; doubt.
+
 
   Lemma M_lock_set [MN0 MN1 a n0 n1] :
     KIS MN0 ->
     (MN0 =(a)=> MN1) ->
-    _of lock MN0 n0 = None ->
-    _of lock MN1 n0 = Some n1 ->
+    lock (MN0 n0) = None ->
+    lock (MN1 n0) = Some n1 ->
     exists v, a = NComm n0 n1 Q (MValP v).
 
   Proof.
@@ -1139,7 +1051,6 @@ Module Type SOUND_F(Import Conf : DETECT_CONF)(Import Params : DETECT_PARAMS(Con
       compat_hsimpl in *; hsimpl_net; doubt.
 
     all:
-      Control.enter (fun _ => consider (h = Rad.Rad_handle) by eauto with LTS);
       destruct s; hsimpl in *; simpl in *; doubt.
 
     - destruct n2 as [? [|]]; simpl in *; doubt.
@@ -1151,8 +1062,8 @@ Module Type SOUND_F(Import Conf : DETECT_CONF)(Import Params : DETECT_PARAMS(Con
   Lemma M_lock_unset [MN0 MN1 a n0 n1] :
     KIS MN0 ->
     (MN0 =(a)=> MN1) ->
-    _of lock MN0 n0 = Some n1 ->
-    _of lock MN1 n0 = None ->
+    lock (MN0 n0) = Some n1 ->
+    lock (MN1 n0) = None ->
     exists v, a = NTau n0 (MActP (Recv (n1, R) v)).
 
   Proof.
@@ -1163,65 +1074,34 @@ Module Type SOUND_F(Import Conf : DETECT_CONF)(Import Params : DETECT_PARAMS(Con
       compat_hsimpl in *; hsimpl_net; doubt.
 
     all:
-      Control.enter (fun _ => consider (h = Rad.Rad_handle) by (eauto with LTS));
       destruct s; hsimpl in *; simpl in *; doubt.
 
     - smash_eq n2 n1; eattac.
     - destruct n2 as [? [|]]; eattac.
       smash_eq n n1; eattac.
       destruct (NAME.eqb (init msg) &self); attac.
-      destruct (&lock_id =? index msg); attac.
+      rewrite next_state_Send_all in *.
+      bs.
   Qed.
-
-
-  (* Lemma SRPC_pq_in_net_in_R_no_out [srpc I P O s v] : *)
-  (*   SRPC_pq_in_net srpc (serv I P O) -> *)
-  (*   List.In (s, R, v) I -> *)
-  (*   O = []. *)
-
-  (* Proof. *)
-  (*   intros. *)
-  (*   enough (forall n t v, ~ List.In (n, t, v) &O) as Hx. *)
-  (*   { *)
-  (*     clear - Hx. *)
-  (*     induction O; intros; auto. *)
-  (*     destruct a as [[n t] v]. *)
-  (*     bs (List.In (n, &t, v) ((n, &t, v)::&O)). *)
-  (*   } *)
-  (*   intros n t v'. *)
-  (*   destruct t. *)
-  (*   - intros ?. *)
-  (*     consider (n = s). *)
-  (*     { *)
-  (*       assert (exists c, srpc = Lock c s) by eauto with LTS. *)
-  (*       assert (exists c, srpc = Lock c n) by eauto with LTS. *)
-  (*       attac. *)
-  (*     } *)
-  (*     bs. *)
-  (*   - consider (exists c, srpc = Lock c s) by eauto with LTS. *)
-  (*     assert (&O = [] \/ &O <> []) as [|] by (destruct O; attac); subst; auto. *)
-  (*     consider (exists v, List.In (s, Q, v) &O) by eauto with LTS. *)
-  (*     bs. *)
-  (* Qed. *)
 
 
   Lemma M_lock_no_send [MN0 MN1 n0 n1 m0 m1 t v] :
     KIS MN0 ->
-    _of lock MN0 n0 = Some n1 ->
+    lock (MN0 n0) = Some n1 ->
     (MN0 =(NComm m0 m1 t (MValP v))=> MN1) ->
     n0 <> m0.
 
   Proof.
     intros.
-    assert (net_lock_on '' MN0 n0 n1 \/ exists v, List.In (TrRecv (n1, R) v) (get_MQ MN0 n0)) as [|]
+    assert (net_lock_on MN0 n0 n1 \/ exists v, List.In (TrRecv (n1, R) v) (mserv_i (MN0 n0))) as [|]
         by eauto with LTS.
     1: eauto using locked_M_no_send with LTS.
 
     intros ?; subst.
     hsimpl in *.
-    unfold get_MQ in *.
+    unfold NetGet in *.
 
-    destruct (NetMod.get m0 '' MN0) as [I0 P0 O0] eqn:?.
+    destruct (NetMod.get m0 ('' MN0)) as [I0 P0 O0] eqn:?.
     assert (List.In (n1, R, v0) I0).
     {
       destruct (NetMod.get m0 MN0) as [MQ0 M0 [I0' P0' O0']] eqn:?.
@@ -1231,7 +1111,7 @@ Module Type SOUND_F(Import Conf : DETECT_CONF)(Import Params : DETECT_PARAMS(Con
 
     consider (O0 = []).
     {
-      consider (net_sane '' MN0) by eauto with LTS.
+      consider (net_sane MN0) by eauto with LTS.
       specialize (H_Sane_SRPC m0) as [srpc Hsrpc].
       hrewrite NetMod.get in *.
       replace O0 with (serv_o (serv I0 P0 O0)) by auto.
@@ -1250,8 +1130,8 @@ Module Type SOUND_F(Import Conf : DETECT_CONF)(Import Params : DETECT_PARAMS(Con
   Lemma M_lock_no_reset [MN0 MN1 a n0 n1 n1'] :
     KIS MN0 ->
     (MN0 =(a)=> MN1) ->
-    _of lock MN0 n0 = Some n1 ->
-    _of lock MN1 n0 = Some n1' ->
+    lock (MN0 n0) = Some n1 ->
+    lock (MN1 n0) = Some n1' ->
     n1' = n1.
 
   Proof.
@@ -1266,49 +1146,49 @@ Module Type SOUND_F(Import Conf : DETECT_CONF)(Import Params : DETECT_PARAMS(Con
       Control.enter (fun _ => consider (_ =(_)=> _));
       ltac1:(autounfold with LTS_get in * );
       compat_hsimpl in *; hsimpl_net; doubt;
-       Control.enter (fun _ => consider (h = Rad.Rad_handle) by eauto with LTS);
        destruct s; hsimpl in *; simpl in *; doubt.
 
     - blast_cases; iattac.
     - destruct n2 as [? [|]]; eattac.
       smash_eq n n1; eattac.
       destruct (NAME.eqb (init msg) &self); attac.
-      destruct (&lock_id =? index msg); attac.
+      rewrite next_state_Send_all in *; attac.
     - bs (NComm n1' n1' Q # v <> NComm n1' n1' Q # v).
     - bs (NComm n0 n1' Q # v <> NComm n0 n1' Q # v).
   Qed.
+
+  Hint Rewrite -> next_state_Send_all : LTS.
 
 
   Lemma M_lock_set_act [MN0 MN1 n0 n1 v] :
     KIS MN0 ->
     (MN0 =(NComm n0 n1 Q (MValP v))=> MN1) ->
-    _of lock MN0 n0 = None /\ _of lock MN1 n0 = Some n1.
+    lock (MN0 n0) = None /\ lock (MN1 n0) = Some n1.
 
   Proof.
     intros.
-    consider (~ net_lock_on '' MN0 n0 n1 /\ net_lock_on '' MN1 n0 n1)
+    consider (~ net_lock_on MN0 n0 n1 /\ net_lock_on MN1 n0 n1)
       by (eauto using SRPC_M_net_query_new_lock with LTS).
 
     split.
-    - enough (forall n, _of lock MN0 n0 <> Some n) by (destruct (_of lock MN0 n0); attac). intros ? ?.
-      apply `(~ net_lock_on '' MN0 _ _).
-      assert (net_lock_on '' MN0 n0 n \/ exists v, List.In (TrRecv (n, R) v) (get_MQ MN0 n0)) as [|]
+    - enough (forall n, lock (MN0 n0) <> Some n) by (destruct (lock (MN0 n0)); attac). intros ? ?.
+      apply `(~ net_lock_on MN0 _ _).
+      assert (net_lock_on MN0 n0 n \/ exists v, List.In (TrRecv (n, R) v) (mserv_i (MN0 n0))) as [|]
           by eauto with LTS.
       + consider (n = n1) by eauto using SRPC_M_net_no_immediate_relock with LTS.
       + hsimpl in *.
 
-        destruct (NetMod.get n0 '' MN0) as [I0 P0 O0] eqn:?.
+        destruct (NetMod.get n0 ('' MN0)) as [I0 P0 O0] eqn:?.
         assert (List.In (n, R, v0) I0).
         {
-          unfold get_MQ in *.
           destruct (NetMod.get n0 MN0) as [MQ0 M0 [I0' P0' O0']] eqn:?.
-          unfold net_deinstr, deinstr in *. hsimpl in *.
+          unfold NetGet, net_deinstr, deinstr in *. hsimpl in *.
           attac.
         }
 
         consider (O0 = []).
         {
-          consider (net_sane '' MN0) by eauto with LTS.
+          consider (net_sane MN0) by eauto with LTS.
           specialize (H_Sane_SRPC n0) as [srpc Hsrpc].
           rewrite `(NetMod.get n0 _ = _) in *.
           replace (O0) with (serv_o (serv I0 P0 O0)) by auto. (* TODO seek and destroy this bs *)
@@ -1323,9 +1203,8 @@ Module Type SOUND_F(Import Conf : DETECT_CONF)(Import Params : DETECT_PARAMS(Con
         bs.
     - consider (_ =(_)=> _).
       compat_hsimpl in *.
-      unfold net_deinstr, deinstr in *.
+      unfold NetGet, net_deinstr, deinstr in *.
       hsimpl in *.
-      consider (h = Rad.Rad_handle) by eauto with LTS.
       destruct s.
       simpl in *.
       smash_eq n0 n1; hsimpl in *; attac.
@@ -1341,17 +1220,17 @@ Module Type SOUND_F(Import Conf : DETECT_CONF)(Import Params : DETECT_PARAMS(Con
   Proof.
     intros.
 
-    destruct (NetMod.get n0 '' MN0) as [I0 P0 O0] eqn:?.
+    destruct (NetMod.get n0 ('' MN0)) as [I0 P0 O0] eqn:?.
     assert (List.In (n1, R, v) I0).
     {
-      unfold get_MQ in *.
+      unfold NetGet in *.
       unfold net_deinstr, deinstr in *. hsimpl in *.
       attac.
     }
 
     consider (O0 = []).
     {
-      consider (net_sane '' MN0) by eauto with LTS.
+      consider (net_sane MN0) by eauto with LTS.
       specialize (H_Sane_SRPC n0) as [srpc Hsrpc].
       rewrite `(NetMod.get n0 _ = _) in *.
       replace (O0) with (serv_o (serv I0 P0 O0)) by auto. (* TODO seek and destroy this bs *)
@@ -1365,13 +1244,13 @@ Module Type SOUND_F(Import Conf : DETECT_CONF)(Import Params : DETECT_PARAMS(Con
 
   Lemma M_R_in_no_send_MM [MN0 n0 n1 v] :
     KIS MN0 ->
-    List.In (TrRecv (n1, R) v) (get_MQ MN0 n0)  ->
-    MQ_s (get_MQ MN0 n0) = [].
+    List.In (TrRecv (n1, R) v) (mserv_i (MN0 n0))  ->
+    MQ_s (mserv_i (MN0 n0)) = [].
 
   Proof.
     intros.
     destruct (NetMod.get n0 MN0) as [MQ0 M0 [I0 P0 O0]] eqn:?.
-    unfold get_MQ in *; hsimpl in *.
+    unfold NetGet in *; hsimpl in *.
     assert (List.In (n1, R, v) (I0 ++ MQ_r MQ0)) by attac.
     assert ((MQ_s MQ0 ++ O0) = []) by eauto using M_R_in_no_send with LTS.
     apply app_eq_nil in H2.
@@ -1423,8 +1302,8 @@ Module Type SOUND_F(Import Conf : DETECT_CONF)(Import Params : DETECT_PARAMS(Con
   Lemma M_wait_add [MN0 MN1 a n0 n1] :
     KIS MN0 ->
     (MN0 =(a)=> MN1) ->
-    ~ List.In n1 (_of waitees MN0 n0) ->
-    List.In n1 (_of waitees MN1 n0) ->
+    ~ List.In n1 (wait (MN0 n0)) ->
+    List.In n1 (wait (MN1 n0)) ->
     exists v, a = NTau n0 (MActP (Recv (n1, Q) v)).
 
   Proof.
@@ -1436,25 +1315,24 @@ Module Type SOUND_F(Import Conf : DETECT_CONF)(Import Params : DETECT_PARAMS(Con
       compat_hsimpl in *; hsimpl_net; doubt.
 
     all:
-      Control.enter (fun _ => consider (h = Rad.Rad_handle) by eauto with LTS);
       destruct s; hsimpl in *; simpl in *; doubt.
 
-    - assert (List.In n1 (n2::&waitees)) by (blast_cases; attac).
+    - assert (List.In n1 (n2::&wait)) by (blast_cases; attac).
       attac.
-    - assert (List.In n1 &waitees) by (blast_cases; attac).
+    - assert (List.In n1 &wait) by (blast_cases; attac).
       bs.
-    - assert (List.In n1 &waitees) by (blast_cases; attac).
-      bs.
-    - bs (List.In n1 &waitees /\ n1 <> n0) by eauto using in_remove.
-    - bs (List.In n1 &waitees /\ n1 <> n2) by eauto using in_remove.
+    - unfold NetGet in *.
+      blast_cases; compat_hsimpl in *; attac.
+    - bs (List.In n1 &wait /\ n1 <> n0) by eauto using in_remove.
+    - bs (List.In n1 &wait /\ n1 <> n2) by eauto using in_remove.
   Qed.
 
 
   Lemma M_wait_remove [MN0 MN1 a n0 n1] :
     KIS MN0 ->
     (MN0 =(a)=> MN1) ->
-    List.In n1 (_of waitees MN0 n0) ->
-    ~ List.In n1 (_of waitees MN1 n0) ->
+    List.In n1 (wait (MN0 n0)) ->
+    ~ List.In n1 (wait (MN1 n0)) ->
     exists v, a = NComm n0 n1 R v.
 
   Proof.
@@ -1466,89 +1344,28 @@ Module Type SOUND_F(Import Conf : DETECT_CONF)(Import Params : DETECT_PARAMS(Con
       compat_hsimpl in *; hsimpl_net; doubt.
 
     all:
-      Control.enter (fun _ => consider (h = Rad.Rad_handle) by eauto with LTS);
       destruct s; hsimpl in *; simpl in *; doubt.
 
-    all: blast_cases; eattac.
-    - smash_eq n1 n0; attac.
-      bs (List.In n1 (List.remove NAME.eq_dec n0 &waitees)) by eauto using in_in_remove.
-
-    - smash_eq n1 n2; attac.
-      bs (List.In n1 (List.remove NAME.eq_dec n2 &waitees)) by eauto using in_in_remove.
-  Qed.
-
-
-  Lemma M_lock_id_update [MN0 MN1 a n0] :
-    KIS MN0 ->
-    (MN0 =(a)=> MN1) ->
-    _of lock_id MN0 n0 <> _of lock_id MN1 n0 ->
-    exists n1 v, a = NComm n0 n1 Q (MValP v).
-
-  Proof.
-    intros.
-
-    destruct_mna a;
-      Control.enter (fun _ => consider (_ =(_)=> _));
-      ltac1:(autounfold with LTS_get in * );
-      compat_hsimpl in *; hsimpl_net; doubt.
-
-    all:
-      Control.enter (fun _ => consider (h = Rad.Rad_handle) by eauto with LTS);
-      destruct s; hsimpl in *; simpl in *; doubt.
-
-    all: blast_cases; eattac.
-  Qed.
-
-
-  Lemma M_lock_id_incr [MN0 MN1 a n0] :
-    KIS MN0 ->
-    (MN0 =(a)=> MN1) ->
-    _of lock_id MN1 n0 = _of lock_id MN0 n0 \/ _of lock_id MN1 n0 = S (_of lock_id MN0 n0).
-
-  Proof.
-    intros.
-
-    destruct_mna a;
-      Control.enter (fun _ => consider (_ =(_)=> _));
-      ltac1:(autounfold with LTS_get in * );
-      compat_hsimpl in *; hsimpl_net; doubt.
-
-    all: eattac.
-    all:
-      Control.enter (fun _ => consider (h = Rad.Rad_handle) by eauto with LTS);
-      destruct s; hsimpl in *; simpl in *; doubt.
-
-    all: blast_cases; eattac.
-  Qed.
-
-
-  Lemma M_lock_id_update_act [MN0 MN1 n0 n1 v] :
-    KIS MN0 ->
-    (MN0 =(NComm n0 n1 Q (MValP v))=> MN1) ->
-    _of lock_id MN1 n0 = S (_of lock_id MN0 n0).
-
-  Proof.
-    intros.
-    consider (_ =(_)=> _).
-    compat_hsimpl in *.
-    ltac1:(autounfold with LTS_get in * ).
-    consider (h = Rad.Rad_handle) by eauto with LTS.
-    hsimpl_net; attac.
+    all: blast_cases; compat_hsimpl in *; eattac.
+    - smash_eq n0 n1; attac.
+      bs (List.In n1 (List.remove NAME.eq_dec n0 &wait)) by eauto using in_in_remove.
+    - smash_eq n1 n2; compat_hsimpl in *; attac.
+      bs (List.In n1 (List.remove NAME.eq_dec n2 &wait)) by eauto using in_in_remove.
   Qed.
 
 
   Lemma M_alarm_set [MN0 MN1 a n0] :
     KIS MN0 ->
     (MN0 =(a)=> MN1) ->
-    _of alarm MN0 n0 = false ->
-    _of alarm MN1 n0 = true ->
+    alarm (MN0 n0) = false ->
+    alarm (MN1 n0) = true ->
     a = NTau n0 (MActM Tau) /\
-      exists n1, List.In (EvRecv (n1, R) {|init:=n0; index:=_of lock_id MN0 n0|}) (get_MQ MN0 n0).
+      exists n1, List.In (EvRecv (n1, R) {|init:=n0|}) (mserv_i (MN0 n0)).
 
   Proof.
     intros.
 
-    assert (_of self MN1 n0 = n0) by eauto using KIS_invariant_self.
+    assert (self (MN1 n0) = n0) by eauto using KIS_invariant_self.
 
     destruct_mna a;
       Control.enter (fun _ => consider (_ =(_)=> _));
@@ -1558,41 +1375,39 @@ Module Type SOUND_F(Import Conf : DETECT_CONF)(Import Params : DETECT_PARAMS(Con
     all: try (destruct msg).
 
     all:
-      Control.enter (fun _ => consider (h = Rad.Rad_handle) by eauto with LTS);
       destruct s; hsimpl in *; simpl in *; doubt.
 
     all: blast_cases; eattac.
-
-    consider (&lock_id = &index) by (apply PeanoNat.Nat.eqb_eq; auto).
-    eauto with LTS.
+    compat_hsimpl in *.
+    bs.
   Qed.
 
 
   Lemma KIS_invariant_lock [MN0 MN1 a] :
     (MN0 =(a)=> MN1) ->
     KIS MN0 ->
-    forall n0 n1, _of lock MN1 n0 = Some n1 -> net_lock_on '' MN1  n0 n1 \/ exists v, List.In (TrRecv (n1, R) v) (get_MQ MN1 n0).
+    forall n0 n1, lock (MN1 n0) = Some n1 -> net_lock_on MN1  n0 n1 \/ exists v, List.In (TrRecv (n1, R) v) (mserv_i (MN1 n0)).
 
   Proof.
     intros.
 
-    destruct (net_sane_lock_dec '' MN1 n0 n1); eauto using KIS_invariant_sane with LTS.
+    destruct (net_sane_lock_dec MN1 n0 n1); eauto using KIS_invariant_sane with LTS.
     right.
 
-    destruct (net_sane_lock_dec '' MN0 n0 n1); eauto with LTS.
+    destruct (net_sane_lock_dec MN0 n0 n1); eauto with LTS.
     - consider (exists v, a = NComm n1 n0 R (MValP v))
         by eauto using SRPC_M_net_unlock_reply with LTS.
-      unfold get_MQ in *.
+      unfold NetGet in *.
       consider (_ =(_)=> _).
-      eattac.
-    - assert (net_sane '' MN0) by eauto with LTS.
-      assert (net_sane '' MN1) by eauto with LTS.
+      compat_hsimpl in *; eattac.
+    - assert (net_sane MN0) by eauto with LTS.
+      assert (net_sane MN1) by eauto with LTS.
 
-      assert ((exists v, List.In (TrRecv (n1, R) v) (get_MQ MN1 n0))
-                              \/ forall v, ~ List.In (TrRecv (n1, R) v) (get_MQ MN1 n0)
+      assert ((exists v, List.In (TrRecv (n1, R) v) (mserv_i (MN1 n0)))
+                              \/ forall v, ~ List.In (TrRecv (n1, R) v) (mserv_i (MN1 n0))
              ) as [|]; auto.
       {
-        generalize (get_MQ MN1 n0) as Q0. clear.
+        generalize (mserv_i (MN1 n0)) as Q0. clear.
         intros.
         induction Q0; attac.
         destruct `(_ \/ _); attac.
@@ -1601,27 +1416,26 @@ Module Type SOUND_F(Import Conf : DETECT_CONF)(Import Params : DETECT_PARAMS(Con
       }
       exfalso.
 
-      destruct (_of lock MN0 n0) as [n1'| ] eqn:?.
+      destruct (lock (MN0 n0)) as [n1'| ] eqn:?.
       + consider (n1' = n1) by (symmetry; eauto using M_lock_no_reset).
-        assert (net_lock_on '' MN0 n0 n1 \/ exists v, List.In (TrRecv (n1, R) v) (get_MQ MN0 n0)) by eauto with LTS.
+        assert (net_lock_on MN0 n0 n1 \/ exists v, List.In (TrRecv (n1, R) v) (mserv_i (MN0 n0))) by eauto with LTS.
         hsimpl in *.
-        unfold get_MQ in *.
+        unfold NetGet in *.
 
         destruct (NetMod.get n0 MN0) as [MQ0 M0 [I0 P0 O0]] eqn:?.
         destruct (NetMod.get n0 MN1) as [MQ1 M1 [I1 P1 O1]] eqn:?.
 
-        destruct_mna a; hsimpl in *.
+        destruct_mna a; compat_hsimpl in *.
 
         all: smash_eq n n0; hsimpl in *.
 
         par: doubt.
 
-        all: hsimpl in *.
+        all: compat_hsimpl in *; unfold NetGet in *.
         * bs (~ In (TrRecv (n1, R) v) (MQ0 ++ [TrSend _ _])) by eauto.
         * bs (~ In (TrRecv (n1, R) v) (MQ0 ++ [TrSend _ _])) by eauto.
         * bs.
         * destruct `(_ \/ _); hsimpl in *; doubt.
-          consider (h = Rad.Rad_handle) by eauto with LTS.
           ltac1:(autounfold with LTS_get in * ).
           hsimpl in *.
           simpl in H1.
@@ -1635,26 +1449,26 @@ Module Type SOUND_F(Import Conf : DETECT_CONF)(Import Params : DETECT_PARAMS(Con
           consider (MN0 =(_)=> _); hsimpl in *.
           hsimpl_net; bs.
         * assert (~ In (TrRecv (n1, R) v) MQ1) by eauto.
-          consider (MN0 =(_)=> _); hsimpl in *.
+          consider (MN0 =(_)=> _); compat_hsimpl in *.
           hsimpl_net; bs.
         * assert (~ In (TrRecv (n1, R) v) MQ1) by eauto.
-          consider (MN0 =(_)=> _); hsimpl in *.
+          consider (MN0 =(_)=> _); compat_hsimpl in *.
           hsimpl_net; bs.
         * assert (~ In (TrRecv (n1, R) v) MQ1) by eauto.
-          consider (MN0 =(_)=> _); hsimpl in *.
+          consider (MN0 =(_)=> _); compat_hsimpl in *.
           hsimpl_net; bs.
         * assert (~ In (TrRecv (n1, R) v) MQ1) by eauto.
-          consider (MN0 =(_)=> _); hsimpl in *.
+          consider (MN0 =(_)=> _); compat_hsimpl in *.
           hsimpl_net; bs.
         * assert (~ In (TrRecv (n1, R) v) MQ1) by eauto.
-          consider (MN0 =(_)=> _); hsimpl in *.
+          consider (MN0 =(_)=> _); compat_hsimpl in *.
           hsimpl_net; bs.
         * assert (~ In (TrRecv (n1, R) v) MQ1) by eauto.
-          consider (MN0 =(_)=> _); hsimpl in *.
+          consider (MN0 =(_)=> _); compat_hsimpl in *.
           hsimpl_net; bs.
 
       + enough (exists v, a = NComm n0 n1 Q (MValP v))
-          by (hsimpl in *; consider (~ net_lock_on '' MN0 n0 n1 /\ net_lock_on '' MN1 n0 n1) by eauto using SRPC_M_net_query_new_lock).
+          by (hsimpl in *; consider (~ net_lock_on MN0 n0 n1 /\ net_lock_on MN1 n0 n1) by eauto using SRPC_M_net_query_new_lock).
 
         eauto using M_lock_set.
   Qed.
@@ -1663,42 +1477,42 @@ Module Type SOUND_F(Import Conf : DETECT_CONF)(Import Params : DETECT_PARAMS(Con
   Lemma KIS_invariant_wait [MN0 MN1 a] :
     (MN0 =(a)=> MN1) ->
     KIS MN0 ->
-    forall n0 n1, List.In n0 (_of waitees MN1 n1) -> net_lock_on '' MN1 n0 n1.
+    forall n0 n1, List.In n0 (wait (MN1 n1)) -> net_lock_on MN1 n0 n1.
 
   Proof.
     intros.
-    destruct (net_sane_lock_dec '' MN1 n0 n1); eauto with LTS.
+    destruct (net_sane_lock_dec MN1 n0 n1); eauto with LTS.
     exfalso.
 
-    destruct (in_dec NAME.eq_dec n0 (_of waitees MN0 n1)).
-    - assert (net_lock_on '' MN0 n0 n1) by eauto with LTS.
+    destruct (in_dec NAME.eq_dec n0 (wait (MN0 n1))).
+    - assert (net_lock_on MN0 n0 n1) by eauto with LTS.
       consider (exists v, a = NComm n1 n0 R (MValP v)) by eauto using SRPC_M_net_unlock_reply with LTS.
 
       consider (_ =(_)=> _).
       compat_hsimpl in *.
       ltac1:(autounfold with LTS_get in * ).
-      consider (h = Rad.Rad_handle) by eauto with LTS.
       destruct s.
       hsimpl_net.
-      + bs (~ List.In n0 (List.remove NAME.eq_dec n0 &waitees)) by eauto using remove_In.
-      + bs (~ List.In n0 (List.remove NAME.eq_dec n0 &waitees)) by eauto using remove_In.
+      + bs (~ List.In n0 (List.remove NAME.eq_dec n0 &wait)) by eauto using remove_In.
+      + bs (~ List.In n0 (List.remove NAME.eq_dec n0 &wait)) by eauto using remove_In.
 
     - rename n into Hn.
       assert (exists v, a = NTau n1 (MActP (Recv (n0, Q) v))) by eauto using M_wait_add with LTS.
 
-      enough (net_lock_on '' MN0 n0 n1).
+      enough (net_lock_on MN0 n0 n1).
       {
         consider (exists v, a = NComm n1 n0 R (MValP v)) by eauto using SRPC_M_net_unlock_reply with LTS.
         bs.
       }
+      enough (pq_client n0 (NetMod.get n1 ('' MN0))) by eauto with LTS.
 
-      destruct (NetMod.get n1 '' MN0) as [I0' P0' O0'] eqn:?.
+      destruct (NetMod.get n1 ('' MN0)) as [I0' P0' O0'] eqn:?.
       destruct (NetMod.get n1 MN0) as [MQ0 M0 [I0 P0 O0]] eqn:?.
 
-      enough (pq_client n0 (NetMod.get n1 '' MN0)) by eauto with LTS.
       enough (exists v, List.In (n0, Q, v) I0') by iattac.
       enough (exists v, List.In (TrRecv (n0, Q) v) MQ0)
-        by (hsimpl in *; exists v0; unfold net_deinstr, deinstr in *; ieattac).
+        by (compat_hsimpl in *; exists v0; unfold net_deinstr, deinstr in *; ieattac).
+      unfold NetGet in *. compat_hsimpl in *.
       eattac.
   Qed.
 
@@ -1732,20 +1546,18 @@ Module Type SOUND_F(Import Conf : DETECT_CONF)(Import Params : DETECT_PARAMS(Con
   Proof.
     intros.
 
-    destruct (NetMod.get n0 MN0) as [MQ0 [h s0] S0] eqn:?.
-    consider (h = Rad.Rad_handle) by eauto with LTS.
-    destruct (NetMod.get n0 MN1) as [MQ1 [h s1] S1] eqn:?.
-    assert (handle (get_M MN1 n0) = Rad_handle) by eauto with LTS.
+    destruct (NetMod.get n0 MN0) as [MQ0 s0 S0] eqn:?.
+    destruct (NetMod.get n0 MN1) as [MQ1 s1 S1] eqn:?.
 
-    destruct_mna a; hsimpl in *.
+    destruct_mna a; compat_hsimpl in *.
 
     all: ltac1:(autounfold with LTS_get in * ); hsimpl_net; blast_cases; eattac.
 
     - consider (MN0 =(_)=> _); hsimpl in *.
       hsimpl_net; doubt.
-    - consider (MN0 =(_)=> _); hsimpl in *.
+    - consider (MN0 =(_)=> _); compat_hsimpl in *.
       hsimpl_net; doubt.
-    - consider (MN0 =(_)=> _); hsimpl in *.
+    - consider (MN0 =(_)=> _); compat_hsimpl in *.
       exfalso.
       hsimpl_net; hsimpl in *; doubt.
       + apply `(~ sends_to_mon _ _ _).
@@ -1758,7 +1570,7 @@ Module Type SOUND_F(Import Conf : DETECT_CONF)(Import Params : DETECT_PARAMS(Con
         destruct (MProbe_eq_dec m p); subst; constructor; attac.
         smash_eq n2 n1.
         attac.
-    - consider (MN0 =(_)=> _); hsimpl in *.
+    - consider (MN0 =(_)=> _); compat_hsimpl in *.
       hsimpl_net; hsimpl in *; doubt.
   Qed.
 
@@ -1766,20 +1578,19 @@ Module Type SOUND_F(Import Conf : DETECT_CONF)(Import Params : DETECT_PARAMS(Con
   Lemma KIS_invariant_sendp [MN0 MN1 a] :
     (MN0 =(a)=> MN1) ->
     KIS MN0 ->
-    forall n0 n1 p, sends_to MN1 n1 n0 p -> net_lock_on '' MN1 n0 n1.
+    forall n0 n1 p, sends_to MN1 n1 n0 p -> net_lock_on MN1 n0 n1.
 
   Proof.
     intros.
 
-    destruct (NetMod.get n1 MN0) as [MQ0 [h0 s0] S0] eqn:?.
-    consider (h0 = Rad.Rad_handle) by eauto with LTS.
+    destruct (NetMod.get n1 MN0) as [MQ0 s0 S0] eqn:?.
 
-    destruct (NetMod.get n1 MN1) as [MQ1 [h1 s1] S1] eqn:?.
+    destruct (NetMod.get n1 MN1) as [MQ1 s1 S1] eqn:?.
 
-    destruct (net_sane_lock_dec '' MN1 n0 n1); eauto with LTS.
+    destruct (net_sane_lock_dec MN1 n0 n1); eauto with LTS.
 
     destruct (sends_to_dec MN0 n1 n0 p).
-    - assert (net_lock_on '' MN0 n0 n1) by eauto with LTS.
+    - assert (net_lock_on MN0 n0 n1) by eauto with LTS.
 
       consider (exists v, a = NComm n1 n0 R (MValP v)) by eauto using SRPC_M_net_unlock_reply with LTS.
 
@@ -1788,111 +1599,38 @@ Module Type SOUND_F(Import Conf : DETECT_CONF)(Import Params : DETECT_PARAMS(Con
 
     - assert ((exists v, a = NTau n1 (MActP (Recv (n0, Q) v))) \/ a = NTau n1 (MActM Tau)) as [|]
           by eauto using M_sends_to_send_set with LTS.
-      + hsimpl in *.
-        enough (net_lock_on '' MN0 n0 n1).
+      + compat_hsimpl in *.
+        enough (net_lock_on MN0 n0 n1).
         {
           consider (exists v', NTau n1 (MActP (Recv (n0, Q) v)) = NComm n1 n0 R (MValP v')) by (eapply SRPC_M_net_unlock_reply; attac; constructor; attac).
           bs.
         }
 
-        enough (pq_client n0 (NetMod.get n1 '' MN0)) by eauto with LTS.
-          enough (List.In (TrRecv (n0, Q) v) (get_MQ MN0 n1))
+        enough (pq_client n0 (NetMod.get n1 ('' MN0))) by eauto with LTS.
+          enough (List.In (TrRecv (n0, Q) v) (mserv_i (MN0 n1)))
           by (ltac1:(autounfold with LTS_get in * ); unfold net_deinstr, deinstr in *; attac).
         ltac1:(autounfold with LTS_get in * ); hsimpl in *.
         blast_cases; attac.
-      + enough (List.In n0 (_of waitees MN1 n1)) by eauto using KIS_invariant_wait.
+      + enough (List.In n0 (wait (MN1 n1))) by eauto using KIS_invariant_wait.
         consider (MN0 =(_)=> _).
-        hsimpl in *.
+        compat_hsimpl in *.
 
         blast_cases; attac.
 
-        par: unfold sends_to in *; ltac1:(autounfold with LTS_get in * ); hsimpl in *; bs.
+        par: unfold NetGet, sends_to in *; ltac1:(autounfold with LTS_get in * ); compat_hsimpl in *; try (rewrite next_state_Send_all); bs.
   Qed.
-
-
-  Lemma KIS_invariant_index_sendp [MN0 MN1 a] :
-    (MN0 =(a)=> MN1) ->
-    KIS MN0 ->
-    forall n0 n1 p, sends_to MN1 n0 n1 p -> (index p <= _of lock_id MN1 (init p))%nat.
-
-  Proof.
-    intros.
-
-    destruct (NetMod.get n0 MN0) as [MQ0 [h s0] S0] eqn:?.
-    consider (h = Rad.Rad_handle) by eauto with LTS.
-    destruct (NetMod.get n0 MN1) as [MQ1 [h s1] S1] eqn:?.
-    assert (handle (get_M MN1 n0) = Rad_handle) by eauto with LTS.
-
-    destruct (sends_to_dec MN0 n0 n1 p).
-    - assert ((index p <= _of lock_id MN0 (init p))%nat) by eauto with LTS.
-      unfold sends_to in *.
-
-      destruct p.
-
-      destruct (NetMod.get &init MN0) as [MQp0 [h' sp0] Sp0] eqn:?.
-      consider (h' = Rad.Rad_handle) by eauto with LTS.
-      destruct (NetMod.get &init MN1) as [MQp1 [h' sp1] Sp1] eqn:?.
-      assert (handle (get_M MN1 n0) = Rad_handle) by eauto with LTS.
-
-      destruct_mna a;
-        consider (MN0 =(_)=> _);
-        ltac1:(autounfold with LTS_get in * );
-        hsimpl in *; hsimpl_net; hsimpl in *; doubt.
-
-      par: simpl in *; blast_cases; ieattac.
-
-    - destruct (NetMod.get (init p) MN0) as [MQp0 [h'' sp0] Sp0] eqn:?.
-      consider (h'' = Rad.Rad_handle) by eauto with LTS.
-      destruct (NetMod.get (init p) MN1) as [MQp1 [h'' sp1] Sp1] eqn:?.
-      assert (handle (get_M MN1 (init p)) = Rad_handle) by eauto with LTS.
-
-      assert ((exists v, a = NTau n0 (MActP (Recv (n1, Q) v))) \/ a = NTau n0 (MActM Tau)) as [|]
-          by eauto using M_sends_to_send_set with LTS.
-      + hsimpl in *.
-        ltac1:(autounfold with LTS_get in * ).
-        hsimpl_net; hsimpl in *.
-        all: blast_cases; attac.
-
-        consider (&self = n0) by eauto with LTS.
-        bs.
-
-      + hsimpl in *.
-
-        unfold sends_to in *; ltac1:(autounfold with LTS_get in * ); hsimpl in *; doubt.
-        all: blast_cases; attac.
-
-
-        hsimpl_net; hsimpl in *.
-        * enough (index p <= _of lock_id MN0 (init p))
-            by (ltac1:(autounfold with LTS_get in * ); hsimpl in *; eattac).
-          enough (List.In (EvRecv (n1, R) p) (get_MQ MN0 (init p))) by eauto with LTS.
-
-          absurd (&self = init p); auto.
-          enough (_of self MN0 (init p) = (init p)) by (ltac1:(autounfold with LTS_get in * ); attac).
-          eauto with LTS.
-        * enough (index p <= _of lock_id MN0 (init p))
-            by (ltac1:(autounfold with LTS_get in * ); hsimpl in *; eattac).
-          eenough (List.In (EvRecv (_, R) p) (get_MQ MN0 n0)) by eauto with LTS.
-
-          enough (&self = n0) by (ltac1:(autounfold with LTS_get in * ); attac).
-
-          enough (_of self MN0 n0 = n0) by (ltac1:(autounfold with LTS_get in * ); attac).
-          eauto with LTS.
-  Qed.
-
 
   Lemma M_recv_ev_act [MN0 MN1 a n0 n1 t p] :
     KIS MN0 ->
     (MN0 =(a)=> MN1) ->
-    ~ List.In (EvRecv (n1, t) p) (get_MQ MN0 n0) ->
-    List.In (EvRecv (n1, t) p) (get_MQ MN1 n0) ->
+    ~ List.In (EvRecv (n1, t) p) (mserv_i (MN0 n0)) ->
+    List.In (EvRecv (n1, t) p) (mserv_i (MN1 n0)) ->
     a = NComm n1 n0 t ^ p.
 
   Proof.
     intros.
 
-    destruct (NetMod.get n0 MN0) as [MQ0 [h s0] S0] eqn:?.
-    consider (h = Rad.Rad_handle) by eauto with LTS.
+    destruct (NetMod.get n0 MN0) as [MQ0 s0 S0] eqn:?.
 
     destruct_mna a;
       Control.enter (fun _ => consider (_ =(_)=> _));
@@ -1901,49 +1639,6 @@ Module Type SOUND_F(Import Conf : DETECT_CONF)(Import Params : DETECT_PARAMS(Con
 
     all: auto.
   Qed.
-
-
-  Lemma KIS_invariant_index_recvp [MN0 MN1 a] :
-    (MN0 =(a)=> MN1) ->
-    KIS MN0 ->
-    forall n0 n1 p, List.In (EvRecv (n1, R) p) (get_MQ MN1 n0) ->
-                                      (index p <= _of lock_id MN1 (init p))%nat.
-
-  Proof.
-    intros.
-
-    assert (handle (get_M MN1 (init p)) = Rad_handle) by eauto with LTS.
-
-    assert (In (EvRecv (n1, R) p) (get_MQ MN0 n0) \/ ~ In (EvRecv (n1, R) p) (get_MQ MN0 n0)) as [|].
-    - induction (get_MQ MN0 n0); attac.
-      destruct `(_ \/ _); attac.
-      destruct a0; attac.
-      destruct n.
-      destruct (MProbe_eq_dec p m); attac.
-      destruct t; attac.
-      smash_eq n n1; attac.
-    - assert (index p <= _of lock_id MN0 (init p)) by eauto with LTS.
-      destruct (PeanoNat.Nat.eq_dec (_of lock_id MN1 (init p)) (_of lock_id MN0 (init p))).
-      1: attac.
-
-      consider (exists n1' v, a = NComm (init p) n1' Q (MValP v)) by eauto using M_lock_id_update.
-
-      consider (_of lock MN0 (init p) = None /\ _of lock MN1 (init p) = Some n1') by eauto using M_lock_set_act.
-      consider (_ =(_)=> _); compat_hsimpl in *.
-      ltac1:(autounfold with LTS_get in * ); hsimpl in *.
-      hsimpl_net; hsimpl in *; doubt.
-      all: blast_cases; attac.
-    - assert (a = NComm n1 n0 R ^ p) by eauto using  M_recv_ev_act.
-      destruct (PeanoNat.Nat.eq_dec (_of lock_id MN1 (init p)) (_of lock_id MN0 (init p))).
-      2: consider (exists n1' v, a = NComm (init p) n1' Q (MValP v)) by (eauto using M_lock_id_update; hsimpl in * ); bs.
-      enough (sends_to MN0 n1 n0 p) by (rewrite `(_of lock_id MN1 _ = _) in *; eauto with LTS).
-
-      subst.
-      consider (_ =(_)=> _); compat_hsimpl in *.
-      unfold sends_to in *; ltac1:(autounfold with LTS_get in * ); hsimpl in *.
-      attac.
-  Qed.
-
 
   Lemma dep_dec_after : forall N0 N1 a n0 n1,
       net_sane N0 ->
@@ -1972,16 +1667,16 @@ Module Type SOUND_F(Import Conf : DETECT_CONF)(Import Params : DETECT_PARAMS(Con
         * consider (a0 = n2) by eauto using SRPC_net_no_relock with LTS.
   Qed.
 
-  Lemma dep_dec_after_M : forall MN0 MN1 ma n0 n1,
-      net_sane '' MN0 ->
-      dep_on '' MN0 n0 n1 ->
+  Lemma dep_dec_after_M : forall (MN0 MN1 : MNet) ma n0 n1,
+      net_sane MN0 ->
+      dep_on MN0 n0 n1 ->
       (MN0 =(ma)=> MN1) ->
-      dep_on '' MN1 n0 n1 \/ ~ dep_on '' MN1 n0 n1.
+      dep_on MN1 n0 n1 \/ ~ dep_on MN1 n0 n1.
 
   Proof.
     intros.
     destruct (MNAct_to_PNAct ma) as [a|] eqn:?.
-    - assert ('' MN0 =(a)=> '' MN1) by eauto using net_deinstr_act_do with LTS.
+    - assert ('' MN0 =(a)=> MN1) by eauto using net_deinstr_act_do with LTS.
       now eauto using dep_dec_after.
     - replace ('' MN1) with ('' MN0) by eauto using net_deinstr_act_skip with LTS.
       now left.
@@ -1991,78 +1686,64 @@ Module Type SOUND_F(Import Conf : DETECT_CONF)(Import Params : DETECT_PARAMS(Con
   Lemma KIS_invariant_recvp_hot [MN0 MN1 a] :
     (MN0 =(a)=> MN1) ->
     KIS MN0 ->
-    forall n0 n1 n2, List.In (hot_ev_of MN1 n1 n2) (get_MQ MN1 n0) ->
-                                  _of lock MN1 n2 <> None ->
-                                  dep_on '' MN1 n0 n2.
+    forall n0 n1 n2, List.In (hot_ev_of n1 n2 ) (mserv_i (MN1 n0)) ->
+                                  lock (MN1 n2) <> None ->
+                                  dep_on MN1 n0 n2.
 
   Proof.
     intros.
 
-    destruct (NetMod.get n0 MN0) as [MQ00 [h0 s00] S00] eqn:?.
-    consider (h0 = Rad.Rad_handle) by eauto with LTS.
-    destruct (NetMod.get n0 MN1) as [MQ01 [h0 s01] S01] eqn:?.
-    assert (handle (get_M MN1 n0) = Rad_handle) by eauto with LTS.
+    destruct (NetMod.get n0 MN0) as [MQ00 s00 S00] eqn:?.
+    destruct (NetMod.get n0 MN1) as [MQ01 s01 S01] eqn:?.
 
-    destruct (NetMod.get n1 MN0) as [MQ10 [h1 s10] S10] eqn:?.
-    consider (h1 = Rad.Rad_handle) by eauto with LTS.
-    destruct (NetMod.get n1 MN1) as [MQ11 [h1 s11] S11] eqn:?.
-    assert (handle (get_M MN1 n1) = Rad_handle) by eauto with LTS.
+    destruct (NetMod.get n1 MN0) as [MQ10 s10 S10] eqn:?.
+    destruct (NetMod.get n1 MN1) as [MQ11 s11 S11] eqn:?.
 
-    destruct (NetMod.get n2 MN0) as [MQ20 [h2 s20] S20] eqn:?.
-    consider (h2 = Rad.Rad_handle) by eauto with LTS.
-    destruct (NetMod.get n2 MN1) as [MQ21 [h2 s21] S21] eqn:?.
-    assert (handle (get_M MN1 n2) = Rad_handle) by eauto with LTS.
+    destruct (NetMod.get n2 MN0) as [MQ20 s20 S20] eqn:?.
+    destruct (NetMod.get n2 MN1) as [MQ21 s21 S21] eqn:?.
 
-    assert (In (hot_ev_of MN1 n1 n2) (get_MQ MN0 n0) \/ ~ In (hot_ev_of MN1 n1 n2) (get_MQ MN0 n0)) as [|].
+    assert (In (hot_ev_of n1 n2 ) (mserv_i (MN0 n0)) \/ ~ In (hot_ev_of n1 n2 ) (mserv_i (MN0 n0))) as [|].
     {
       unfold hot_ev_of. clear.
-      induction (get_MQ MN0 n0); attac.
+      induction (mserv_i (MN0 n0)); attac.
       destruct `(_ \/ _); attac.
       destruct a; attac.
       destruct n.
-      destruct (MProbe_eq_dec (hot_of MN1 n2) m); attac.
+      destruct (MProbe_eq_dec (hot_of n2) m); attac.
       destruct t; attac.
       smash_eq n n1; attac.
     }
     2: {
       unfold hot_ev_of in *.
-      consider (a = NComm n1 n0 R ^ (hot_of MN1 n2)) by eauto using M_recv_ev_act.
-      assert (sends_to MN0 n1 n0 (hot_of MN1 n2)).
+      consider (a = NComm n1 n0 R ^ (hot_of n2)) by eauto using M_recv_ev_act.
+      assert (sends_to MN0 n1 n0 (hot_of n2)).
       {
-        remember (hot_of MN1 n2) as p; clear - H.
+        remember (hot_of n2) as p; clear - H.
         consider (_ =(_)=> _); compat_hsimpl in *.
         unfold sends_to; ltac1:(autounfold with LTS_get in * ); attac.
       }
-      consider (net_lock_on '' MN0 n0 n1 /\ net_lock_on '' MN1 n0 n1).
+      consider (net_lock_on MN0 n0 n1 /\ net_lock_on MN1 n0 n1).
       {
-        assert (net_lock_on '' MN0 n0 n1) by eauto with LTS.
+        assert (net_lock_on MN0 n0 n1) by eauto with LTS.
         split; auto.
-        destruct (net_sane_lock_dec '' MN1 n0 n1); eauto with LTS.
-        consider (exists v, NComm n1 n0 R ^ (hot_of MN1 n2) = NComm n1 n0 R (MValP v)) by eauto using SRPC_M_net_unlock_reply with LTS.
+        destruct (net_sane_lock_dec MN1 n0 n1); eauto with LTS.
+        consider (exists v, NComm n1 n0 R ^ (hot_of n2) = NComm n1 n0 R (MValP v)) by eauto using SRPC_M_net_unlock_reply with LTS.
         bs.
       }
-      assert (_of lock MN0 n2 <> None).
+      assert (lock (MN0 n2) <> None).
       {
         intros ?.
-        destruct (_of lock MN1 n2) as [n3|] eqn:?; doubt.
-        consider (exists v, NComm n1 n0 R ^ (hot_of MN1 n2) = NComm n2 n3 Q (MValP v)) by eauto using M_lock_set.
+        destruct (lock (MN1 n2)) as [n3|] eqn:?; doubt.
+        consider (exists v, NComm n1 n0 R ^ (hot_of n2) = NComm n2 n3 Q (MValP v)) by eauto using M_lock_set.
       }
-      assert (hot_of MN1 n2 = hot_of MN0 n2).
-      {
-        enough (_of lock_id MN1 n2 = _of lock_id MN0 n2) by (unfold hot_of; attac).
-        destruct (PeanoNat.Nat.eq_dec (_of lock_id MN1 n2) (_of lock_id MN0 n2)); auto.
-        consider (exists n3' v, NComm n1 n0 R ^ (hot_of MN1 n2) = NComm n2 n3' Q (MValP v)) by eauto using M_lock_id_update.
-        bs.
-      }
-      rewrite `(hot_of _ _ = _) in *.
 
-      assert (dep_on '' MN0 n0 n2) by eauto with LTS.
+      assert (dep_on MN0 n0 n2) by eauto with LTS.
 
-      enough ('' MN0 = '' MN1) by attac.
+      enough ('' MN0 = MN1) by attac.
       eapply net_deinstr_act_skip; attac.
     }
 
-    destruct (_of lock MN1 n2) as [n3|] eqn:?. 2: doubt.
+    destruct (lock (MN1 n2)) as [n3|] eqn:?. 2: doubt.
 
     assert ((exists v, a = NComm n2 n3 Q (MValP v)) \/ forall v, a <> NComm n2 n3 Q (MValP v)) as [|].
     {
@@ -2070,41 +1751,60 @@ Module Type SOUND_F(Import Conf : DETECT_CONF)(Import Params : DETECT_PARAMS(Con
       destruct_mna a; try (solve [left; eexists; eattac | right; eattac ]).
       smash_eq n n0 n2 n3; try (solve [left; eexists; eattac | right; eattac ]).
     }
-    - assert (_of lock_id MN0 n2 < _of lock_id MN1 n2).
+    - 
+
+      unfold NetGet in *.
+      eattac.
+      enough (dep_on MN0 n0 n2).
       {
-        hsimpl in *.
-        assert (_of lock_id MN1 n2 = S (_of lock_id MN0 n2)) by eauto using M_lock_id_update_act.
-        lia.
+        unshelve eapply net_deinstr_act_do in H; attac.
+        eauto 2 using net_dep_Q_preserve with LTS.
+      }
+      consider (KIS _).
+      eapply H_recvp_hot_S.
+      unfold NetGet in *.
+      rewrite `(NetMod.get n0 MN0 = _).
+      attac.
+      eauto with LTS.
+      enough (dep_on MN0 n1 n2).
+      {
+        smash_eq n0 n1.
+        enough (net_lock_on MN0 n0 n1) by eauto with LTS.
+
+        consider (KIS _).
+
+        unshelve eapply net_deinstr_act_do in H; attac.
+        eauto 2 using net_dep_Q_preserve with LTS.
       }
 
-      enough (_of lock_id MN1 n2 <= _of lock_id MN0 n2) by lia.
-      enough (index (hot_of MN1 n2) <= _of lock_id MN0 (init (hot_of MN1 n2))) by (simpl in *; lia).
+
       eauto with LTS.
 
-    - assert (_of lock_id MN0 n2 = _of lock_id MN1 n2).
+
+    - assert (lock_id (MN0 n2) = lock_id (MN1 n2)).
       {
-        destruct (PeanoNat.Nat.eq_dec (_of lock_id MN0 n2) (_of lock_id MN1 n2)) as [He|He]; auto.
+        destruct (PeanoNat.Nat.eq_dec (lock_id (MN0 n2)) (lock_id (MN1 n2))) as [He|He]; auto.
         consider (exists n3' v, a = NComm n2 n3' Q (MValP v)) by eauto using M_lock_id_update.
-        consider (_of lock MN0 n2 = None /\ _of lock MN1 n2 = Some n3') by eauto using M_lock_set_act.
+        consider (lock (MN0 n2) = None /\ lock (MN1 n2) = Some n3') by eauto using M_lock_set_act.
         attac.
       }
-      replace (hot_ev_of MN1 n1 n2) with (hot_ev_of MN0 n1 n2) by (unfold hot_ev_of, hot_of; attac).
-      assert (_of lock MN0 n2 = Some n3).
+      replace (hot_ev_of n1 n2 ) with (hot_ev_of n1 n2 ) by (unfold hot_ev_of, hot_of; attac).
+      assert (lock (MN0 n2) = Some n3).
       {
-        destruct (_of lock MN0 n2) as [n3'|] eqn:?.
+        destruct (lock (MN0 n2)) as [n3'|] eqn:?.
         - enough (n3 = n3') by attac.
           eauto using M_lock_no_reset.
         - consider (exists v, a = NComm n2 n3 Q (MValP v)) by eauto using M_lock_set.
           bs.
       }
-      assert (dep_on '' MN0 n0 n2) by (assert (_of lock MN0 n2 <> None) by attac; eauto with LTS).
-      assert (dep_on '' MN1 n0 n2 \/ ~ dep_on '' MN1 n0 n2) as [|]; eauto using dep_dec_after_M with LTS.
+      assert (dep_on MN0 n0 n2) by (assert (lock (MN0 n2) <> None) by attac; eauto with LTS).
+      assert (dep_on MN1 n0 n2 \/ ~ dep_on MN1 n0 n2) as [|]; eauto using dep_dec_after_M with LTS.
 
-      consider (exists n0' v, (n0 = n0' \/ dep_on '' MN1 n0 n0') /\ a = NComm n2 n0' R (MValP v)).
+      consider (exists n0' v, (n0 = n0' \/ dep_on MN1 n0 n0') /\ a = NComm n2 n0' R (MValP v)).
       {
         destruct (MNAct_to_PNAct a) eqn:?.
-        - assert ('' MN0 =(p)=> '' MN1) by eauto using net_deinstr_act_do with LTS.
-          consider (exists n0' v, p = NComm n2 n0' R v /\ (n0' = n0 \/ dep_on '' MN1 n0 n0')).
+        - assert ('' MN0 =(p)=> MN1) by eauto using net_deinstr_act_do with LTS.
+          consider (exists n0' v, p = NComm n2 n0' R v /\ (n0' = n0 \/ dep_on MN1 n0 n0')).
           {
             eapply net_dep_on_unlock with (n0:=n0)(n1:=n2)(N1:=''MN1)(N0:=''MN0); eauto with LTS.
           }
@@ -2125,52 +1825,46 @@ Module Type SOUND_F(Import Conf : DETECT_CONF)(Import Params : DETECT_PARAMS(Con
   Lemma KIS_invariant_sendp_hot [MN0 MN1 a] :
     (MN0 =(a)=> MN1) ->
     KIS MN0 ->
-    (forall n0 n1 n2, sends_to MN1 n1 n0 (hot_of MN1 n2) -> _of lock MN1 n2 <> None -> dep_on '' MN1 n0 n2).
+    (forall n0 n1 n2, sends_to MN1 n1 n0 (hot_of n2) -> lock (MN1 n2) <> None -> dep_on MN1 n0 n2).
 
   Proof.
     intros.
 
-    destruct (NetMod.get n0 MN0) as [MQ00 [h0 s00] S00] eqn:?.
-    consider (h0 = Rad.Rad_handle) by eauto with LTS.
-    destruct (NetMod.get n0 MN1) as [MQ01 [h0 s01] S01] eqn:?.
-    assert (handle (get_M MN1 n0) = Rad_handle) by eauto with LTS.
+    destruct (NetMod.get n0 MN0) as [MQ00 s00 S00] eqn:?.
+    destruct (NetMod.get n0 MN1) as [MQ01 s01 S01] eqn:?.
 
-    destruct (NetMod.get n1 MN0) as [MQ10 [h1 s10] S10] eqn:?.
-    consider (h1 = Rad.Rad_handle) by eauto with LTS.
-    destruct (NetMod.get n1 MN1) as [MQ11 [h1 s11] S11] eqn:?.
-    assert (handle (get_M MN1 n1) = Rad_handle) by eauto with LTS.
+    destruct (NetMod.get n1 MN0) as [MQ10 s10 S10] eqn:?.
+    destruct (NetMod.get n1 MN1) as [MQ11 s11 S11] eqn:?.
 
-    destruct (NetMod.get n2 MN0) as [MQ20 [h2 s20] S20] eqn:?.
-    consider (h2 = Rad.Rad_handle) by eauto with LTS.
-    destruct (NetMod.get n2 MN1) as [MQ21 [h2 s21] S21] eqn:?.
-    assert (handle (get_M MN1 n2) = Rad_handle) by eauto with LTS.
+    destruct (NetMod.get n2 MN0) as [MQ20 s20 S20] eqn:?.
+    destruct (NetMod.get n2 MN1) as [MQ21 s21 S21] eqn:?.
 
-    assert (net_lock_on '' MN1 n0 n1) by eauto using KIS_invariant_sendp.
+    assert (net_lock_on MN1 n0 n1) by eauto using KIS_invariant_sendp.
 
-    destruct (sends_to_dec MN0 n1 n0 (hot_of MN1 n2)) as [|].
+    destruct (sends_to_dec MN0 n1 n0 (hot_of n2)) as [|].
     2: {
       assert ((exists v, a = NTau n1 (MActP (Recv (n0, Q) v))) \/ a = NTau n1 (MActM Tau))
         by eauto using M_sends_to_send_set with LTS.
 
-      assert (_of lock MN0 n2 <> None).
+      assert (lock (MN0 n2) <> None).
       {
         intros ?.
-        destruct (_of lock MN1 n2) as [n3|] eqn:?; doubt.
+        destruct (lock (MN1 n2)) as [n3|] eqn:?; doubt.
         consider (exists v, a = NComm n2 n3 Q (MValP v)) by eauto using M_lock_set.
         destruct `(_ \/ _); bs.
       }
-      assert (hot_of MN1 n2 = hot_of MN0 n2).
+      assert (hot_of n2 = hot_of n2).
       {
-        enough (_of lock_id MN1 n2 = _of lock_id MN0 n2) by (unfold hot_of; attac).
-        destruct (PeanoNat.Nat.eq_dec (_of lock_id MN1 n2) (_of lock_id MN0 n2)); auto.
+        enough (lock_id (MN1 n2) = lock_id (MN0 n2)) by (unfold hot_of; attac).
+        destruct (PeanoNat.Nat.eq_dec (lock_id (MN1 n2)) (lock_id (MN0 n2))); auto.
         consider (exists n3' v, a = NComm n2 n3' Q (MValP v)) by eauto using M_lock_id_update.
         destruct `(_ \/ _); bs.
       }
       rewrite `(hot_of _ _ = _) in *.
 
-      assert (net_lock_on '' MN0 n0 n1).
+      assert (net_lock_on MN0 n0 n1).
       {
-        destruct (net_sane_lock_dec '' MN0 n0 n1); auto with LTS.
+        destruct (net_sane_lock_dec MN0 n0 n1); auto with LTS.
         consider (exists v, a = NComm n0 n1 Q (MValP v)) by eauto using SRPC_M_net_new_lock_query with LTS.
         destruct `(_ \/ _); bs.
       }
@@ -2179,30 +1873,30 @@ Module Type SOUND_F(Import Conf : DETECT_CONF)(Import Params : DETECT_PARAMS(Con
       - hsimpl in *.
         enough (n2 = n1) by attac 2.
         consider (_ =(_)=> _); compat_hsimpl in * |-.
-        assert (_of self MN0 n1 = n1) by eauto with LTS.
+        assert (self (MN0 n1) = n1) by eauto with LTS.
         unfold hot_ev_of, hot_of in *; ltac1:(autounfold with LTS_get in * ).
         destruct &lock.
         consider (sends_to_mon _ _ _); attac 2.
         consider (sends_to_mon _ _ _).
         bs.
-      - assert (dep_on '' MN0 n0 n2).
+      - assert (dep_on MN0 n0 n2).
         {
-          enough (dep_on '' MN0 n1 n2) by attac.
-          enough (exists n', List.In (hot_ev_of MN0 n' n2) (get_MQ MN0 n1)) by (hsimpl in *; eauto with LTS).
+          enough (dep_on MN0 n1 n2) by attac.
+          enough (exists n', List.In (hot_ev_of (n' n2)) (mserv_i (MN0 n1))) by (hsimpl in *; eauto with LTS).
           unfold hot_ev_of, hot_of, sends_to in *.
           ltac1:(autounfold with LTS_get in * ); hsimpl in *.
           consider (_ =(_)=> _); compat_hsimpl in *.
           blast_cases; attac.
         }
 
-        assert (dep_on '' MN1 n0 n2 \/ ~ dep_on '' MN1 n0 n2) as [|] by eauto using dep_dec_after_M with LTS; auto.
+        assert (dep_on MN1 n0 n2 \/ ~ dep_on MN1 n0 n2) as [|] by eauto using dep_dec_after_M with LTS; auto.
 
-        assert (exists m0 m1 v, (n0 = m0 \/ dep_on '' MN0 n0 m0) /\ NTau n1 (MActM Tau) = NComm m1 m0 R (MValP v)).
+        assert (exists m0 m1 v, (n0 = m0 \/ dep_on MN0 n0 m0) /\ NTau n1 (MActM Tau) = NComm m1 m0 R (MValP v)).
         {
           subst.
           destruct (MNAct_to_PNAct (NTau n1 (MActM Tau))) eqn:?.
-          - assert ('' MN0 =(p)=> '' MN1) by eauto using net_deinstr_act_do with LTS.
-            consider (exists n0' v, p = NComm n2 n0' R v /\ (n0' = n0 \/ dep_on '' MN1 n0 n0')).
+          - assert ('' MN0 =(p)=> MN1) by eauto using net_deinstr_act_do with LTS.
+            consider (exists n0' v, p = NComm n2 n0' R v /\ (n0' = n0 \/ dep_on MN1 n0 n0')).
             {
               eapply net_dep_on_unlock with (n0:=n0)(n1:=n2)(N1:=''MN1)(N0:=''MN0); eauto with LTS.
             }
@@ -2213,7 +1907,7 @@ Module Type SOUND_F(Import Conf : DETECT_CONF)(Import Params : DETECT_PARAMS(Con
         hsimpl in *; bs.
     }
 
-    destruct (_of lock MN1 n2) as [n3|] eqn:?. 2: doubt.
+    destruct (lock (MN1 n2)) as [n3|] eqn:?. 2: doubt.
 
     assert ((exists v, a = NComm n2 n3 Q (MValP v)) \/ forall v, a <> NComm n2 n3 Q (MValP v)) as [|].
     {
@@ -2221,41 +1915,41 @@ Module Type SOUND_F(Import Conf : DETECT_CONF)(Import Params : DETECT_PARAMS(Con
       destruct_mna a; try (solve [left; eexists; eattac | right; eattac ]).
       smash_eq n n0 n2 n3; try (solve [left; eexists; eattac | right; eattac ]).
     }
-    - assert (_of lock_id MN0 n2 < _of lock_id MN1 n2).
+    - assert (lock_id (MN0 n2) < lock_id (MN1 n2)).
       {
         hsimpl in *.
-        assert (_of lock_id MN1 n2 = S (_of lock_id MN0 n2)) by eauto using M_lock_id_update_act.
+        assert (lock_id (MN1 n2) = S (lock_id (MN0 n2))) by eauto using M_lock_id_update_act.
         lia.
       }
 
-      enough (_of lock_id MN1 n2 <= _of lock_id MN0 n2) by lia.
-      enough (index (hot_of MN1 n2) <= _of lock_id MN0 (init (hot_of MN1 n2))) by (simpl in *; lia).
+      enough (lock_id (MN1 n2) <= lock_id (MN0 n2)) by lia.
+      enough (index (hot_of n2) <= _of lock_id MN0 (init (hot_of n2))) by (simpl in *; lia).
       eauto with LTS.
-    - assert (_of lock_id MN0 n2 = _of lock_id MN1 n2).
+    - assert (lock_id (MN0 n2) = lock_id (MN1 n2)).
       {
-        destruct (PeanoNat.Nat.eq_dec (_of lock_id MN0 n2) (_of lock_id MN1 n2)) as [He|He]; auto.
+        destruct (PeanoNat.Nat.eq_dec (lock_id (MN0 n2)) (lock_id (MN1 n2))) as [He|He]; auto.
         consider (exists n3' v, a = NComm n2 n3' Q (MValP v)) by eauto using M_lock_id_update.
-        consider (_of lock MN0 n2 = None /\ _of lock MN1 n2 = Some n3') by eauto using M_lock_set_act.
+        consider (lock (MN0 n2) = None /\ lock (MN1 n2) = Some n3') by eauto using M_lock_set_act.
         attac.
       }
-      replace (hot_of MN1 n2) with (hot_of MN0 n2) by (unfold hot_of; attac).
-      assert (_of lock MN0 n2 = Some n3).
+      replace (hot_of n2) with (hot_of n2) by (unfold hot_of; attac).
+      assert (lock (MN0 n2) = Some n3).
       {
-        destruct (_of lock MN0 n2) as [n3'|] eqn:?.
+        destruct (lock (MN0 n2)) as [n3'|] eqn:?.
         - enough (n3 = n3') by attac.
           eauto using M_lock_no_reset.
         - consider (exists v, a = NComm n2 n3 Q (MValP v)) by eauto using M_lock_set.
           bs.
       }
-      assert (dep_on '' MN0 n0 n2) by (assert (_of lock MN0 n2 <> None) by attac; eauto with LTS).
+      assert (dep_on MN0 n0 n2) by (assert (lock (MN0 n2) <> None) by attac; eauto with LTS).
 
-      assert (dep_on '' MN1 n0 n2 \/ ~ dep_on '' MN1 n0 n2) as [|] by eauto using dep_dec_after_M with LTS; auto.
+      assert (dep_on MN1 n0 n2 \/ ~ dep_on MN1 n0 n2) as [|] by eauto using dep_dec_after_M with LTS; auto.
 
-      consider (exists n0' v, (n0 = n0' \/ dep_on '' MN1 n0 n0') /\ a = NComm n2 n0' R (MValP v)).
+      consider (exists n0' v, (n0 = n0' \/ dep_on MN1 n0 n0') /\ a = NComm n2 n0' R (MValP v)).
       {
         destruct (MNAct_to_PNAct a) eqn:?.
-        - assert ('' MN0 =(p)=> '' MN1) by eauto using net_deinstr_act_do with LTS.
-          consider (exists n0' v, p = NComm n2 n0' R v /\ (n0' = n0 \/ dep_on '' MN1 n0 n0')).
+        - assert ('' MN0 =(p)=> MN1) by eauto using net_deinstr_act_do with LTS.
+          consider (exists n0' v, p = NComm n2 n0' R v /\ (n0' = n0 \/ dep_on MN1 n0 n0')).
           {
             eapply net_dep_on_unlock with (n0:=n0)(n1:=n2)(N1:=''MN1)(N0:=''MN0); eauto with LTS.
           }
@@ -2276,27 +1970,26 @@ Module Type SOUND_F(Import Conf : DETECT_CONF)(Import Params : DETECT_PARAMS(Con
   Lemma KIS_invariant_alarm [MN0 MN1 a] :
     (MN0 =(a)=> MN1) ->
     KIS MN0 ->
-    forall n, _of alarm MN1 n = true -> dep_on '' MN1 n n.
+    forall n, alarm (MN1 n) = true -> dep_on MN1 n n.
 
   Proof.
     intros.
-    destruct (NetMod.get n MN0) as [MQ [h s] S] eqn:?.
-    consider (h = Rad.Rad_handle) by eauto with LTS.
+    destruct (NetMod.get n MN0) as [MQ s S] eqn:?.
 
-    enough (dep_on '' MN0 n n).
+    enough (dep_on MN0 n n).
     {
-      assert (deadlocked n '' MN0) by (eauto using dep_self_deadlocked with LTS).
+      assert (deadlocked n MN0) by (eauto using dep_self_deadlocked with LTS).
       eauto 3 using deadlocked_M_dep_invariant1 with LTS.
     }
 
-    destruct (_of alarm MN0 n) eqn:?; eauto 2 with LTS.
+    destruct (alarm (MN0 n)) eqn:?; eauto 2 with LTS.
 
     consider (a = NTau n (MActM Tau) /\
-                exists n1, List.In (EvRecv (n1, R) {|init:=n; index:=_of lock_id MN0 n|}) (get_MQ MN0 n)) by eauto using M_alarm_set.
+                exists n1, List.In (EvRecv (n1, R) {|init:=n; index:=lock_id (MN0 n)|}) (mserv_i (MN0 n))) by eauto using M_alarm_set.
 
-    assert (List.In (hot_ev_of MN0 n1 n) (get_MQ MN0 n)) by eauto with LTS.
+    assert (List.In (hot_ev_of n1 n ) (mserv_i (MN0 n))) by eauto with LTS.
 
-    enough (_of lock MN0 n <> None) by eauto with LTS.
+    enough (lock (MN0 n) <> None) by eauto with LTS.
 
     consider (_ =(_)=> _); compat_hsimpl in *.
     ltac1:(autounfold with LTS_get in * ); hsimpl in *.
@@ -2313,7 +2006,6 @@ Module Type SOUND_F(Import Conf : DETECT_CONF)(Import Params : DETECT_PARAMS(Con
       eauto using
         KIS_invariant_sane
       , KIS_invariant_self
-      , KIS_invariant_Rad
       , KIS_invariant_lock
       , KIS_invariant_wait
       , KIS_invariant_sendp
@@ -2330,22 +2022,22 @@ Module Type SOUND_F(Import Conf : DETECT_CONF)(Import Params : DETECT_PARAMS(Con
 
   Lemma KIS_detection [MN n] :
     KIS MN ->
-    _of alarm MN n = true ->
-    exists DS, DeadSet DS '' MN /\ In n DS.
+    alarm (MN n) = true ->
+    exists DS, DeadSet DS MN /\ In n DS.
 
   Proof.
     intros.
     enough (deadlocked n MN) by (consider (deadlocked _ _); attac).
-    enough (dep_on '' MN n n) by eauto using dep_self_deadlocked with LTS.
+    enough (dep_on MN n n) by eauto using dep_self_deadlocked with LTS.
     consider (KIS MN).
   Qed.
 
 
   Theorem detection_soundness [i0 N0 MN1 mpath n] :
-    KIS (net_instr i0 N0) ->
-    (net_instr i0 N0 =[mpath]=> MN1) ->
-    _of alarm MN1 n = true ->
-    exists DS, DeadSet DS '' MN1 /\ In n DS.
+    KIS (i0 N0) ->
+    (i0 N0 =[mpath]=> MN1) ->
+    alarm (MN1 n) = true ->
+    exists DS, DeadSet DS MN1 /\ In n DS.
 
   Proof.
     intros.
@@ -2367,7 +2059,7 @@ Module Type SOUND_F(Import Conf : DETECT_CONF)(Import Params : DETECT_PARAMS(Con
       destruct a; kill Heqo; blast_cases; doubt; hsimpl in |- *.
       + Print Serv_Transp_M.
         Print MNAct_to_PNAct.
-        assert ('' MN0 =(p)=> '' N1). eapply net_deinstr_act_do. 2: eauto. simpl in *. eauto.
+        assert ('' MN0 =(p)=> N1). eapply net_deinstr_act_do. 2: eauto. simpl in *. eauto.
         attac.
         {
           constructor. eauto with LTS.
@@ -2382,12 +2074,12 @@ Module Type SOUND_F(Import Conf : DETECT_CONF)(Import Params : DETECT_PARAMS(Con
           kill H2.
           kill H3.
           hsimpl in *.
-          rewrite H in *.
+          rewrite in *.
           unfold deinstr in *.
           eauto.
         }
 
-      + assert ('' MN0 =(p)=> '' N1). eapply net_deinstr_act_do. 2: eauto. simpl in *. eauto.
+      + assert ('' MN0 =(p)=> N1). eapply net_deinstr_act_do. 2: eauto. simpl in *. eauto.
         attac.
         kill H2.
         kill H1.
@@ -2446,12 +2138,12 @@ Module Type SOUND_F(Import Conf : DETECT_CONF)(Import Params : DETECT_PARAMS(Con
   (* TODO: make it into a normal relation? *)
 
 
-  Corollary detection_soundness_instr [N0 i0 MN1 mpath0 n] :
-    KIS (net_instr i0 N0) ->
-    (net_instr i0 N0 =[ mpath0 ]=> MN1) ->
-    _of alarm MN1 n = true ->
+  Corollary detection_soundness_instr [N0 : PNet] [i0 : instr] [MN1 mpath0 n] :
+    KIS (i0 N0) ->
+    (i0 N0 =[ mpath0 ]=> MN1) ->
+    alarm (MN1 n) = true ->
     exists mpath1 i1 N1 DS,
-      (MN1 =[mpath1]=> net_instr i1 N1)
+      (MN1 =[mpath1]=> i1 N1)
       /\ (N0 =[ mpath0 ++ mpath1 ]=> N1)
       /\ In n DS
       /\ DeadSet DS N1.
@@ -2459,16 +2151,16 @@ Module Type SOUND_F(Import Conf : DETECT_CONF)(Import Params : DETECT_PARAMS(Con
   Proof.
     intros.
 
-    consider (exists mpath1 path i2 N2, (MN1 =[ mpath1 ]=> net_instr i2 N2) /\ (N0 =[ path ]=> N2)) by eauto using Net_Transp_soundness.
-    assert ('' (net_instr i0 N0) =[mpath0 ++ mpath1]=> '' (net_instr i2 N2)) by eauto using MNPath_do with LTS.
+    consider (exists mpath1 path i2 N2, (MN1 =[ mpath1 ]=> i2 N2) /\ (N0 =[ path ]=> N2)) by eauto using Net_Transp_soundness.
+    assert ('' (i0 N0) =[mpath0 ++ mpath1]=> (i2 N2)) by eauto using MNPath_do with LTS.
 
     hsimpl in *.
 
-    consider (exists DS, DeadSet DS '' MN1 /\ In n DS) by eauto using detection_soundness.
+    consider (exists DS, DeadSet DS MN1 /\ In n DS) by eauto using detection_soundness.
 
-    assert (DeadSet DS '' (net_instr i2 N2)).
+    assert (DeadSet DS (i2 N2)).
     {
-      consider (exists ppath, '' MN1 =[ppath]=> '' (net_instr i2 N2)) by eauto using Net_path_corr.
+      consider (exists ppath, MN1 =[ppath]=> (i2 N2)) by eauto using Net_path_corr.
       attac.
     }
 
